1. 
$$
\left.\begin{gathered}
\lim\limits_{ n \to +\infty} x_n=a\\
\lim\limits_{ n \to +\infty} y_{n}=b 
\end{gathered}\right| \implies \lim\limits_{ n \to +\infty} (x_n+y_{n})=a+b 
$$
2. $$
\left.\begin{gathered}
\lim\limits_{ n \to +\infty} x_n=a\\
\lim\limits_{ n \to +\infty} y_{n}=b 
\end{gathered}\right| \implies \lim\limits_{ n \to +\infty} (x_ny_{n})=ab 
$$
3. $$
\left.\begin{gathered}
\lim\limits_{ n \to +\infty} x_n=a\\
\lim\limits_{ n \to +\infty} y_{n}=b \ne0
\end{gathered}\right| \implies \lim\limits_{ n \to +\infty} \left(\frac{x_{n}}{y_{n}} \right)=\frac{a}{b} 
$$
4. $\lim\limits_{ n \to +\infty} x_n=a\implies \lim\limits_{ n \to +\infty} |x_{n}| = |a|$
# Док-во
## Пункт 1

fix $\varepsilon>0\implies \exists N\ \forall n\geq N: |x_{n}-a|< \frac{\varepsilon}{2}\text{ и } |y_{n}-b|< \frac{\varepsilon}{2}\implies$
$$
\implies |(x_{n}+y_{n})-(a+b)|=|(x_{n}-a)+(y_{n}-b)|\leq |x_{n}-a|+|y_{n}-b|\leq \varepsilon\implies
$$
$$
\implies \lim\limits_{ n \to +\infty} (x_n+y_{n})=a+b 
$$
## Пункт 2

$x_{n}y_{n}=(a+\alpha_{n})(b+\beta_{n}) = ab + a\beta_{n}+b\alpha_{n} + \alpha_{n}\beta_{n} = ab+\gamma_{n} \Leftrightarrow \lim\limits_{ n \to +\infty} x_ny_{n} = ab$
где $\alpha_{n}, \beta_{n}, \gamma_{n}$ — б/м

## Пункт 3

$\lim\limits_{ n \to +\infty} y_{n} = b\ne0 \implies \text{НСНМ } y_{n}\ne 0\implies \text{НСНМ } \frac{x_{n}}{y_{n}} \text{ опред. НСНМ}$

$\lim\limits_{ n \to +\infty} \frac{x_n}{y_{n}}=\lim\limits_{ n \to +\infty} x_n\frac{1}{y_{n}}$

Хочу д-ть, что $\lim\limits_{ n \to +\infty} \frac{1}{y_{n}}=\frac{1}{b}$

$$
\frac{1}{y_{n}}-\frac{1}{b}=\frac{1}{b+\beta_{n}}-\frac{1}{b}=\frac{b-b-\beta_{n}}{b(b+\beta_{n})}=-\beta_{n} \frac{1}{b(b+\beta_{n})}
$$

НСНМ $|\beta_{n}|= \frac{|b|}{2}$:

$$
|b(b+\beta_{n})|=|b|\cdot|b+\beta_{n}|\leq |b|\cdot\left( |b|+ \frac{|b|}{2} \right)\leq k
$$

$$
|b|\cdot|b+\beta_{n}|\geq |b|\cdot(|b|-|\beta_{n}|) \geq |b|\cdot \frac{|b|}{2}\geq M > 0
$$

$$
\begin{gathered}
0<M\leq|b(b+\beta_{n})|\leq k\\
\frac{1}{k} \leq \frac{1}{b(b+\beta_{n})}\leq \frac{1}{M}\\
\frac{1}{b(b+\beta_{n})}\text{ — огр.} \implies (-\beta_{n})\frac{1}{b(b+\beta_{n})}\text{ — б/м} \implies \lim\limits_{ n \to +\infty} \frac{1}{y_{n}}=\frac{1}{b}\implies \lim\limits_{ n \to +\infty} x_n \frac{1}{y_{n}}=\frac{a}{b}  
\end{gathered}
$$

## Пункт 4

$$
\begin{gathered}
\lim\limits_{ n \to +\infty} x_n=a\\
x_{n}=a+\alpha_{n}\\
|a|-|\alpha_{n}|\leq |x_{n}| \leq |a|+|\alpha_{n}|\\
\Downarrow \text{по П2М} \\
\lim\limits_{ n \to +\infty} |x_n| = |a| 
\end{gathered}
$$
