$a_{i}=\frac{1}{n}\sum\limits_{j=0}^{n-1}b_{j}\varepsilon^{-ij}=\frac{1}{n}g(\varepsilon^{-i}),\ g=\sum\limits_{i=0}^{n-1} b_{i}x^{i}$

## Док-во

$$
\begin{gathered}
b_{i}=\sum\limits_{j=0}^{n-1}a_{j}\varepsilon^{ij}\ |\cdot\varepsilon^{-ij_{0}}\\
b_{i}\varepsilon^{-ij_{0}}=\sum\limits_{j=0
}^{n-1}a_{j}\varepsilon^{i(j-j_{0})}\ |\forall i=0\dots n-1\text{ сложим}\\
\sum\limits_{i=0}^{n-1}b_{i}\varepsilon^{-ij_{0}}=\sum\limits_{i,j=0\dots n-1}a_{j}\varepsilon^{i(j-j_{0})}=\\=\sum\limits_{j=0}^{n-1}a_{j}\sum\limits_{i=0}^{n-1}\varepsilon^{i(j-j_{0})}= \sum\limits_{j=0}^{n-1}a_{j}\sum\limits_{z\in \mu _{n}}z^{j-j_{0}}=\sum\limits_{j=0}^{n-1}a_{j}\begin{cases}
0,\ |j-j_{0}|\ne 0\\
n,\ |j-j_{0}|=0
\end{cases}=\\
=a_{j_{0}}n\implies a_{j_{0}}=\frac{1}{n}\sum\limits_{i=0}^{n-1}b_{i}\varepsilon^{-ij_{0}}
\end{gathered}
$$
