В начале строим $v_{i}^{j}$ — порожд. система, т.ч. $\forall i: \{ v_{i}^{j} \}$ — жорд. цепочка.

Пусть $\{ v_{i}^{j} \}$ — ЛЗ. $\sum\limits a_{ij}v_{i}^{j}=0$. НУО все $i$ разл.: $\sum\limits_{i}a_{is_{i}}v_{i}^{s_{i}}=0$. $\sum\limits a_{is_{i}}\mathscr{A}^{s_{i}}(v_{i}^{0})=0$. НУО $s_{1}$ — мин. из $s_{i}$. Тогда $\sum\limits a_{is_{i}}\mathscr{A}^{s_{1}}(\mathscr{A}^{s_{i}-s_{1}})(v_{i}^{0})=\mathscr{A}^{s_{1}}\left( \sum\limits a_{is_{i}}\mathscr{A}^{s_{i}-s_{1}}v_{i}^{0}\right)=0$. $\sum\limits_{i=1} a_{is_{i}}\mathscr{A}^{s_{i}-s_{1}}(v_{i}^{0})=a_{1s_{1}}v_{1}^{0}+\sum\limits_{i=2} a_{is_{i}}\underbrace{ A^{s_{i}-s_{1}}(v_{i}^{0}) }_{ (v_{1}^{0})_{new} }$. $\mathscr{A}^{s_{1}}(v_{1}^{0})\neq0$, $\mathscr{A}^{s_{1}}(v_{1}^{0})_{new}$ — цепочка укоротилась $\implies$ кол-во $\{ v_{i}^{j} \}$ уменьш. Это всё ещё порожд. сист. Надо проверить $(v_{i}^{j})_{old} \in \langle (v_{i}^{j})_{new} \rangle$. 