$\lambda$ — ед-е с.ч. $\mathscr{A}$ ($\mathscr{A}:V\to V$, $V$ над алг. замкнутым полем, например — $\mathbb{C}$).

Тогда $\mathscr{A}-\lambda\cdot Id$

$$
\begin{gathered}
\mathscr{A}X=\mu X\\
\Updownarrow \\
(\mathscr{A}-\lambda\cdot Id)X=(\mu-\lambda)X
\end{gathered}
$$
Тогда у $\mathscr{A}-\lambda\cdot Id$ — ед-е с.ч. $0\implies (\mathscr{A}-\lambda \cdot Id)$ — нильп, то есть сущ-ет базис, где
$$
\begin{gathered}
[\mathscr{A}-\lambda\cdot Id]=\begin{pmatrix}
\Im_{k_{1}}(0) & 0 \\ 0 & \Im_{k_{2}}(0)\\ 0&0&\dots
\end{pmatrix}\implies\\\implies[\mathscr{A}]=\begin{pmatrix}
\Im_{k_{1}}(\lambda) \\ 0 & \Im_{k_{2}}(\lambda)\\0&0&\dots
\end{pmatrix}
\end{gathered}
$$
где $\Im_{k}(\mu)=\begin{pmatrix}\mu & 0 &0 \\ 1 & \mu & 0\\ 0 & 1 & \mu\\&&&\dots\end{pmatrix}_{k}$

