$f \in C^{2}[\alpha, \beta]$

Тогда 
$$
\Delta:= \int\limits_{\alpha}^{\beta}f(x)\,dx-(\beta-\alpha)\cdot \frac{f(\alpha)+f(\beta)}{2}= -\frac{1}{2}\int\limits_{\alpha}^{\beta} f''(t)(t-\alpha)(\beta-t)\,dt
$$
## Док-во

$\gamma = \frac{\alpha+\beta}{2}$, $u=f,\ v=x-\gamma$

$$
\begin{gathered}
\int\limits_{\alpha}^{\beta} f(x)\,dx=\int\limits_{\alpha}^{\beta} f(x)(x-\gamma)'\,dx=\underbrace{ f(x)(x-\gamma)\bigg|_{x=\alpha}^{x=\beta} }_{ \frac{f(\beta)+f(\alpha)}{2}(\beta-\alpha) }-\int\limits_{\alpha}^{\beta} f'(x)(x-\gamma)\,dx
\end{gathered}
$$
$$
\begin{gathered}
-\int\limits_{\alpha}^{\beta} f'(x)(x-\gamma)\,dx=\left[ \begin{gathered}
u=f',\ v'=x-\gamma\\
v=-\frac{1}{2}(x-\alpha)(\beta-x)=\\=-\frac{1}{2}(-x^{2}+(\alpha+\beta)x-\alpha\beta)
\end{gathered} \right] =\\
=\underbrace{ f'(x)\cdot \left( -\frac{1}{2}(x-\alpha)(\beta-x) \right)\bigg|_{x=\alpha}^{x=\beta} }_{ =0 }-\int\limits_{\alpha}^{\beta} f''(x)\cdot \frac{1}{2}(x-\alpha)(\beta-x)\,dx
\end{gathered}
$$

