$S=\sum\limits_{k=1}^{n}(x_{k}-x_{k-1}) \frac{f(x_{k-1})+f(x_{k})}{2}$

Как выглядит ф-ла, если узлы на равных расстояниях $x_{k}-x_{k-1}=\frac{b-a}{n}$. 
$$
S= \frac{b-a}{n}\cdot \sum\limits_{k=1}^{n} \frac{f(x_{k-1})+f(x_{k})}{2}=\frac{b-a}{n}\left( \frac{f(a)}{2}+\sum\limits_{k=1}^{n}f(x_{k})+\frac{f(b)}{2} \right)
$$
Как выглядит интегральная сумма, если узлы на равных расстояниях и $\xi_{k}=x_{k}$
$$
S(f, \tau, \xi)=\sum\limits_{k=1}^{n} f(\xi_{k})(x_{k}-x_{k-1})=\frac{b-a}{n}\cdot \sum\limits_{k=1}^{n} f(x_{k})
$$
А если $\xi_{k}=x_{k-1}$, то $S(f, \tau, \xi)=\frac{b-a}{n}\cdot \sum\limits_{k=0}^{n-1}f(x_{k})$
>[!note] Если $|f'|\leq M$, то $\omega_{f}(\delta)\leq M\delta$.
> $$
> \left|S(f, \xi, \tau)-\int\limits_{a}^{b} f\right|\leq (b-a)\omega_{f}\left( \frac{b-a}{n} \right)\leq (b-a)^{2}\cdot \frac{M}{n}
> $$
