Заметим, что $n!=\prod\limits_{k=1}^{n}k=\prod\limits_{k=1}^{n}e^{\ln k}=e^{\sum\limits_{k=1}^{n}\ln k}$
$$
\sum\limits_{k=1}^{n}\ln k= \frac{\ln1+\ln n}{2}+\int\limits_{1}^{n} \ln x\,dx-\frac{1}{2}\int\limits_{1}^{n} \frac{\{ x \}(1-\{ x \})}{x^{2}}\,dx\stackrel{(*)}{=}
$$
$f(x)=\ln x, f''(x)= -\frac{1}{x^{2}}$

$$
\int\limits_{1}^{n} \ln x\,dx=(x\ln x-x)\bigg|_{1}^{n}=n\ln n-n+1
$$
$$
\stackrel{(*)}{=}n\ln n-n+\frac{\ln n}{2}+1-\frac{1}{2}\overbrace{ \int\limits_{1}^{n} \left( \frac{\{ x \}(1-\{ x \})}{x^{2}} \right)\,dx }^{ =:b_{n} }\stackrel{(.)}{=}
$$
$b_{n+1}\geq b_{n}$ и 
$$
b_{n} \leq \int\limits_{1}^{n} \frac{dx}{4x^{2}}= -\frac{1}{4x}\bigg|_{1}^{n}=\frac{1}{4}-\frac{1}{4n}< \frac{1}{4}
$$
Т.е. сущ-ет $\lim\limits_{ n \to \infty }b_{n}=b\implies b_{n}=b+o(1)$
$$
\stackrel{(.)}{=}n\ln n-n +\frac{\ln n}{2}+1-\frac{b}{2}+o(1)
$$
Тогда ($e^{o(1)}=1+o(1)$):
$$
n! = n^{n}\cdot e^{-n}\sqrt{n}\cdot e^{1-b/2}\cdot e^{o(1)}=Cn^{n}e^{-n}(1+o(1))\sim Cn^{n}e^{-n}\sqrt{n}
$$
## Чему равна C

$n!\sim Cn^{n}e^{-n}\sqrt{n}$

Знаем, что $\binom{2n}{n}\sim \frac{4^{n}}{\sqrt{\pi n}}$
$$
\binom{2n}{n}=\frac{(2n)!}{(n!)^{2}}\sim \frac{C(2n)^{2n}e^{-2n}\sqrt{2n}}{(Cn^{n}e^{-n}\sqrt{n})^{2}}=\frac{\cancel{ C }4^{n}\cancel{ n^{2n} }\cancel{ e^{-2n} }\sqrt{2\cancel{ n }}}{C^{\cancel{ 2 }}\cancel{ n^{2n} }\cancel{ e^{-2n} }\sqrt{n}\cdot \cancel{ \sqrt{n} }}=\frac{4^{n}\sqrt{2}}{C\sqrt{n}}
$$
$$
\frac{4^{n}}{\sqrt{\pi n}}\sim \frac{4^{n}\sqrt{2}}{C\sqrt{n}}\implies \frac{1}{\sqrt{\pi}}\sim \frac{\sqrt{2}}{C}\implies C=\sqrt{2\pi}
$$
## Формула

Итого, формула имеет вид $n!\sim n^{n}e^{-n}\sqrt{2\pi n}$

>[!note] Чуть более аккуратное рассуждение даёт формулу $n! = n^{n}e^{-n}\sqrt{2\pi n}\cdot e^{O(1/n)}=$ $n^{n}e^{-n}\sqrt{2\pi n}\left( 1+O\left( \frac{1}{n} \right) \right)$

