$f \in C^{2}[m,n];\ m,n \in \mathbb{Z}$

$$
\begin{gathered}
\sum\limits_{k=m}^{n}f(k)=\frac{f(m)+f(n)}{2}+\int\limits_{m}^{n} f(t)\,dt+\frac{1}{2}\int\limits_{m}^{n} f''(t)\{ t \}(1-\{ t \})\,dt
\end{gathered}
$$
# Док-во

Пишем [[Лемма об интеграле через вторую производную|Lm]] для $\alpha=k,\ \beta=k+1$ 
$$
\int\limits_{k}^{k+1} f= \frac{f(k)+f(k+1)}{2}-\frac{1}{2}\int\limits_{k}^{k+1}f''(t)(\overbrace{ t-k }^{ =\{ t \} })(\underbrace{ k+1-t }_{ =1-\{ t \} })\,dt 
$$

Просуммируем по $k$ от $m$ до $n-1$

$$
\underbrace{ \sum\limits_{k=m}^{n-1}\int\limits_{k}^{k+1}f }_{ \int\limits_{m}^{n} f }=\underbrace{ \sum\limits_{k=m}^{n-1}  \frac{f(k)+f(k+1)}{2} }_{ \frac{f(m)}{2}+\sum\limits_{k=m+1}^{n-1}f(k) + \frac{f(n)}{2} }-\frac{1}{2}\underbrace{ \sum\limits_{k=m}^{n-1}\int\limits_{k}^{k+1} f''(t)\{ t \}(1-\{ t \})dt }_{ \int\limits_{m}^{n} f''(t)\{ t \}(1-\{ t \}) }
$$
$$
\int\limits_{m}^{n}f + \frac{f(m)+f(n)}{2}=\sum\limits_{k=m}^{n}f(k)-\frac{1}{2}\int\limits_{m}^{n} f''(t)\{ t \}(1-\{ t \})dt 
$$
