$f, g: \langle a, b \rangle\to \mathbb{R};\ x_{0}\in \langle a,b \rangle;\ f,g$ — дифф. в т. $x_{0}$

Тогда 
1. $f\pm g$ — дифф. в т. $x_{0}$, причём $(f\pm g)'=f'\pm g'$
2. $f\cdot g$ — дифф. в т. $x_{0}$, причём $(f\pm g)'=f'g +g'f$
3. если $g(x_{0})\ne 0$, то $\left( \frac{f}{g} \right)$ — дифф в т. $x_{0}$, причём $\left( \frac{f}{g} \right)'=\frac{f'g-fg'}{g^{2}}$
## Док-во
### Пункт 1

$f$ — дифф. в т. $x_{0} \Leftrightarrow \exists \phi(x):\langle a,b \rangle\to \mathbb{R},\ \phi(x)$ непр. в т. $x_{0}$:
$$
f(x)=f(x_{0})+\phi(x)(x-x_{0})\ \forall x \in \langle a, b \rangle 
$$

$g$ — дифф. в т. $x_{0} \Leftrightarrow \exists \psi(x):\langle a,b \rangle\to \mathbb{R},\ \psi(x)$ непр. в т. $x_{0}$:
$$
g(x)=g(x_{0})+\psi(x)(x-x_{0})\ \forall x \in \langle a, b \rangle 
$$
$$
\begin{gathered}
f(x)\pm g(x)=(f(x_{0})\pm g(x_{0}))+\underbrace{ (\phi(x)\pm \psi(x)) }_{ \text{непр в т.} x_{0} }(x-x_{0})\implies\\\implies f(x)\pm g(x)\text{ дифф. в т. }x_{0}
\end{gathered}
$$
$$
(f(x)\pm g(x))'(x_{0})=\phi(x_{0})\pm\psi(x_{0})=f'(x_{0})\pm g'(x_{0})
$$
### Пункт 2

$$
\begin{gathered}
f(x)g(x)=(f(x_{0})+\phi(x)(x-x_{0}))(g(x_{0})+\psi(x)(x-x_{0}))=\\
=f(x_{0})g(x_{0})+f(x_{0})\psi(x)(x-x_{0})+\phi(x)(x-x_{0})g(x_{0})+\\
+\phi(x)\psi(x)(x-x_{0})^{2}=f(x_{0})g(x_{0})+\\
+\underbrace{ (f(x_{0})\psi(x)+\phi(x)g(x_{0})+\phi(x)\psi(x)(x-x_{0})) }_{ =\xi(x),\ \text{непр. в т. }x_{0} }(x-x_{0})
\end{gathered}
$$
$\xi:\langle a,b \rangle\to \mathbb{R},\ \xi(x)$ — непр. в т. $x_{0}$

$$
\begin{gathered}
f(x)g(x)=f(x_{0})g(x_{0})+\xi(x)(x-x_{0})\stackrel{\text{кр. дифф.}}{\implies}\\
\implies fg\text{ - дифф. в т.} x_{0}\text{ и }(fg)'(x_{0})=\xi(x_{0})=f(x_{0})\psi(x_{0})+\phi(x_{0})g(x_{0})+0=\\=f(x_{0})g'(x_{0})+f'(x_{0})g(x_{0})
\end{gathered}
$$
### Пункт 3

$\left( \frac{f}{g} \right)'=\left( f\cdot \frac{1}{g} \right)'$

$$
\begin{gathered}
\left( \frac{1}{g} \right)'(x_{0})\stackrel{\text{def}}{=}\lim\limits_{ x_ \to x_{0} } \frac{ \frac{1}{g(x)}-\frac{1}{g(x_{0})} }{x-x_{0}}=\lim\limits_{ x \to x_{0} } \frac{g(x_{0})-g(x)}{g(x)g(x_{0})(x-x_{0})}=\\=\lim\limits_{ x \to x_{0} } \underbrace{ \frac{g(x_{0})-g(x)}{x-x_{0}} }_{ \to (-g'(x_{0})) }\cdot \underbrace{ \frac{1}{g(x)} }_{ \text{непр}\implies \to \frac{1}{g(x_{0})} }\cdot \frac{1}{g(x_{0})\ne 0}=\\
=- \frac{g'(x_{0})}{g^{2}(x_{0})}
\end{gathered}
$$
$$
\begin{gathered}
\left( \frac{f}{g} \right)(x_{0})=\left( f\cdot \frac{1}{g} \right)'(x_{0})\stackrel{2}{=}f'(x_{0}) \cdot\frac{1}{g(x_{0})}+f(x_{0})\cdot\left( \frac{1}{g} \right)'(x_{0})=\\
=\frac{f'(x_{0})}{g(x_{0})}-\frac{f(x_{0})g'(x_{0})}{g^{2}(x_{0})}=\frac{f'(x_{0})g(x_{0})-f(x_{0})g'(x_{0})}{g^{2}(x_{0})}
\end{gathered}
$$