$f: \langle a,b \rangle\to \langle m,M \rangle, f$ — строг монот, непр. на $\langle a,b \rangle$
$x_{0} \in \langle a,b \rangle: f'(x_{0})\ne 0$ ($f$ дифф в т. $x_{0}$)

Тогда $f^{-1}$ дифф. в т. $y_{0}=f(x_{0})$ и $(f^{-1})'(y_{0})=\frac{1}{f'(x_{0})}$

## Док-во

$\exists f^{-1}$, более того, $f^{-1}$ — непр. (по [[Теорема об обратных функциях]])

$f$ — дифф в т. $x_{0}\implies \underbrace{ f(x) }_{ y }=\underbrace{ f(x_{0}) }_{ y_{0} }+\phi(x)(x-x_{0}),\ \phi(x)$ непр в т. $x_{0}$
$$
\begin{gathered}
y=f(x)\implies x=f^{-1}(y)\\
y_{0}=f(x_{0})\implies x_{0}=f^{-1}(y_{0})\\
\end{gathered}
$$
$$

y=y_{0}+\phi(f^{-1}(y))(f^{-1}(y)-f^{-1}(y_{0}))\implies y-y_{0}=\phi(f^{-1}(y))(f^{-1}(y)-f^{-1}(y-y_{0}))
$$$$
f^{-1}(y)-f^{-1}(y_{0})=\frac{1}{\underbrace{ \phi(f^{-1}(y)) }_{ \text{непр в т.} y_{0} }\ne 0}(y-y_{0})\stackrel{\text{кр. диф-ти}}{\implies}f^{-1}\text{ дифф. в т. }y_{0}
$$
$$
(f^{-1})'(y_{0})=\frac{1}{\phi(f^{-1}(y_{0}))}=\frac{1}{\phi(x_{0})}=\mathbf{\frac{1}{f'(x_{0})}}=\frac{1}{f'(f^{-1}(y_{0}))}
$$
