$f: \langle a,b \rangle\to \mathbb{R};\ g:\langle c,d \rangle\to \langle a,b \rangle,\ x_{0}\in \langle c,d \rangle;\ y_{0}=g(x_{0})\in \langle a,b \rangle$
$g$ — дифф. в т. $x_{0}$, $f$ — дифф. в т. $y_{0}$

Тогда $f(g)$ — дифф в т. $x_{0}$ и $(f(g))'(x_{0})=f'(y_{0})g'(x_{0})$
## Док-во

$g$ — дифф в т. $x_{0}\stackrel{\text{кр. дифф.}}{\Leftrightarrow}\exists \psi(x):$
$$
g(x)=g(x_{0})+\psi(x)(x-x_0);\ \psi\text{ непр. в т. }x_{0}
$$
$f$ — дифф в т. $y_{0}\stackrel{\text{кр. дифф.}}{\Leftrightarrow}\exists \phi(x):$
$$
f(y)=f(y_{0})+\phi(x)(y-y_0);\ \phi\text{ непр.в т. }y_{0}
$$
$\begin{array}{l}g\text{ - непр в т } x_{0}\\ \phi\text{ - непр в т }x_{0}\\g(x_{0})=y_{0}\end{array}\implies \phi(g(x))\text{ - непр в т.} x_{0}\text{ (непр. композиции)}$

$$
\begin{gathered}
f(g(x))=f(g(x_{0}))+\phi(g(x))\cdot(g(x)-g(x_{0}))=f(g(x_{0}))+\underbrace{ \phi(x)\psi(x) }_{ \xi(x) }(x-x_{0})\\
f(g(x))=f(g(x_{0}))+\xi(x)(x-x_{0})\stackrel{\text{кр. д-ти}}{\implies}f(g(x))\text{ - дифф. в т.} x_{0}
\end{gathered}
$$
$(f(g(x)))'(x_{0})=\xi(x_{0})=\phi(g(x_{0}))\psi(x_{0})=f'(g(x_{0}))\cdot g'(x_{0})=f'(y_{0})g'(x_{0})$

