$f: \langle a, b \rangle\to \mathbb{R};\ x_{0} \in \langle a, b \rangle$

След. усл-я равносильны:
1. $f$ — дифф. в т. $x_{0}$
2. $\exists$ конечн. произв. в т. $x_{0}$
3. $\exists \phi: \langle a,b \rangle\to \mathbb{R}:f(x)-f(x_{0})=\phi(x)(x-x_{0})\ \forall x,\ \phi$ непр. в т. $x_{0}$

Причём, если усл-я вып-ся, то $k = f'(x_{0})=\phi(x_{0})$
## Док-во

### $1\implies 2$

$$
\begin{gathered}
f(x)=f(x_{0})+k(x-x_{0})+o(x-x_{0})\\
\frac{f(x)-f(x_{0})}{x-x_{0}}=k+\frac{o(x-x_{0})}{x-x_{0}}\\
f'(x_{0})=\lim\limits_{ x \to x_{0} }  \frac{f(x)-f(x_{0})}{x-x_{0}}=\lim\limits_{ x \to x_{0} } \left( k+ \cancelto{ 0 }{ \frac{o(x-x_{0})}{x-x_{0}} } \right)=k
\end{gathered}
$$
### $2\implies 3$

$$
\phi(x):= \begin{cases}
\frac{f(x)-f(x_{0})}{x-x_{0}},\ x\ne x_{0}\\
f'(x_{0}),\ x=x_{0}
\end{cases}
$$
### $3\implies 1$

$$
\begin{gathered}
f(x)-f(x_{0})=\phi(x)(x-x_{0})\\
f(x)=f(x_{0})+\phi(x_{0})(x-x_{0})-\phi(x_{0})(x-x_{0})+\phi(x)(x-x_{0})=\\
=f(x_{0})+\phi(x_{0})(x-x_{0})+\underbrace{ (\phi(x)-\phi(x_{0})) }_{ \stackrel{x\to x_{0}}{\to}0 }(x-x_{0})=\\
=f(x_{0})+\phi(x_{0})(x-x_{0})+o(x-x_{0})
\end{gathered}
$$
