1. $c\in \mathbb{R}: (c)'=0$
2. $(x^{p})'=px^{p-1},\ x>0,\ p \in\mathbb{R}$
3. $(a^{x})'=a^{x}\ln a,\ a>0,\ a\ne 1$
4. $(\ln x)'=\frac{1}{x}$
5. $(\sin x)'=\cos x$
6. $(\cos x)'=-\sin x$
7. $(\tg x)'=\frac{1}{\cos ^{2}x}$
8. $(\ctg x)'=-\frac{1}{\sin ^{2}x}$
9. $(\arcsin x)'=\frac{1}{\sqrt{1-x^{2}}}$
10. $(\arccos x)'=-\frac{1}{\sqrt{1-x^{2}}}$
11. $(\arctg x)'=\frac{1}{1+x^{2}}$
12. $(\arcctg x)'=-\frac{1}{1+x^{2}}$
## Док-во
### Пункт 2

$$
\lim\limits_{ h \to 0 } \frac{(x+h)^{p}-x^{p}}{h}=\lim\limits_{ h \to 0 } \frac{ x^{p}\overbrace{ \left( \left( 1+\frac{h}{x} \right)^{p}-1 \right) }^{ \sim p\cdot \frac{h}x } }{h}=\lim\limits_{ h \to 0 } \frac{x^{p}\cdot p\cdot \frac{\cancel{ h }}{x}}{\cancel{ h }}=p\cdot x^{p-1}
$$
### Пункт 3

$$
\lim\limits_{ h \to 0 }  \frac{a^{x+h}-a^{x}}{h}=a^{x}\lim\limits_{ h \to 0 } \frac{a^{h-1}}{h}=a^{x}\ln a
$$
### Пункт 4

$$
(\ln x)'=\frac{\lim\limits_{ h \to 0 }(\ln(x+h)-\ln x)}{h}=\lim\limits_{ h \to 0 } \frac{\ln\left( x+\frac{h}{x} \right)}{h}=\lim\limits_{ h \to 0 } \frac{\overbrace{ \ln\left( 1+\frac{h}{x} \right) }^{ \sim \frac{h}x }}{h}=\lim\limits_{ h \to 0 } \frac{\frac{h}{x}}{h}=\frac{1}{x}
$$

### Пункт 5

$$
\begin{gathered}
(\sin x)'=\lim\limits_{ h \to 0 } \frac{\sin(x+h)-\sin x}{h}=\lim\limits_{ h \to 0 } \frac{2\sin \frac{x+h-x}{2}\cdot \cos \frac{x+h+x}{2}}{h}=\\=\lim\limits_{ h \to 0 } \frac{2\sin \frac{h}{2}\cdot \cos \left( x+\frac{h}{2} \right)}{h}=\lim\limits_{ h \to 0 } \underbrace{ \frac{\sin \frac{h}{2}}{\frac{h}{2}} }_{ \to 1 }\cdot \cos\left( x+\frac{h}{2} \right)=\cos x
\end{gathered}
$$
### Пункт 6

$$
(\cos x)'=\left( \sin\left( x+\frac{\pi}{2} \right) \right)'=\cos\left( \frac{\pi}{2}+x \right)\left( \frac{\pi}{2}+x \right)'=\cos\left( \frac{\pi}{2}+x \right)=-\sin x
$$

### Пункт 7

$$
(\tg x)'=\left( \frac{\sin x}{\cos x} \right)'=\frac{(\sin x)'\cos x-\sin x(\cos x)'}{\cos ^{2}}=\frac{\cos ^{2}x+\sin ^{2}x}{\cos ^{2}x}=\frac{1}{\cos ^{2}x}
$$
### Пункт 8

$\ctg x=\frac{1}{\tg x}$

### Пункт 9

$$
(\arcsin x)'=(\sin ^{-1})'(x)=\frac{1}{\cos\underbrace{ (\arcsin x) }_{ \left[ -\frac{\pi}{2}; \frac{\pi}{2} \right] }}=\frac{1}{\sqrt{1-\sin ^{2}(\arcsin x)}}=\frac{1}{\sqrt{1-x^{2}}}
$$
### Пункт 10

$\arcsin x+\arccos x=\frac{\pi}{2}$
### Пункт 11
$$
(\arctg x)'=(\tg ^{-1})'(x)=\frac{1}{\frac{1}{\cos ^{2}(\arctg x)}}=\cos ^{2}(\arctg x)=\frac{1}{1+\tg ^{2}(\arctg x)}=\frac{1}{1+x^{2}}
$$
### Пункт 12

$\arctg x+\arcctg x=\frac{\pi}{2}$
