(обобщение [[Частная производная]] для высших порядков)

Обозначим
$$
\frac{ \partial^{2} f }{ \partial x_{i}\partial x_{j} }:= \frac{ \partial  }{ \partial x_{i} } \left( \frac{ \partial f }{ \partial x_{j} }  \right) 
$$
$$
f''_{x_{j}x_{i}}:= (f'_{x_{j}})'_{x_{i}}
$$

Если существует $\frac{ \partial^{r}f }{ \partial x_{i_{k}} \partial x_{i_{k-1}}\dots\partial x_{i_{i_{1}}} }$, то у неё можно рассм. произв., т.е. $\frac{ \partial d^{r+1} }{ \partial x_{i_{k+1}}\partial x_{i_{k}}\dots\partial x_{i_{1}} }$

>[!note]- Всего част. произв. порядка $r$ будет $n^{r}$

## Пример

$f(x,y)=x^{y},\ f'_{x}=yx^{y-1},\ f'_{y}=(x^{y}\ln x)$

$$
\begin{array}{l}
f''_{xx}=(yx^{y-1})_{x}'=y(y-1)x^{y-2}& f'_{yy}=(x^{y}\ln x)'_{y}=x^{y}(\ln x)^{2}\\
f''_{xy}=(yx^{y-1})'_{y}=x^{y-1}+yx^{y-1}\ln x & f'_{yx}=(x^{y}\ln x)'_{x}=yx^{y-1}\ln x+\frac{x^{y}}{x}=f''_{xy}
\end{array}
$$

$f(x,y)=\begin{cases} \frac{x^{2}-y^{2}}{x^{2}+y^{2}}\text{ при }(x,y)\neq (0,0)\\0\text{ при }(x,y)=(0,0)\end{cases}$

$$
\begin{gathered}
f'_{x}(x,y)=\frac{3x^{2}y-y^{3}-2x(x^{3}y-xy^{3})}{(x^{2}+y^{2})^{2}}=\\
=\frac{\cancel{ 3 }x^{4}y+3x^{2}y^{3}-\cancel{ x^{2}y^{3} }-y^{5}-\cancel{ 2x^{4} }y+\cancel{ 2 }x^{2}y^{3}}{(x^{2}+y^{2})^{2}}=\frac{x^{4}y+4x^{2}y^{3}-y^{5}}{(x^{2}+y^{2})^{2}}
\end{gathered}
$$
$(x,y)\neq (0,0)$
$$
f'_{x}(0,0)=\lim\limits_{ h \to 0 } \frac{f(h,0)-f(0,0)}{h}=\lim\limits_{ h \to 0 } \frac{0-0}{h}=0
$$
$$
f''_{xy}(0,0)=\lim\limits_{ h \to 0 } \frac{f'_{x}(0,h)-f_{x}'(0,0)}{h}=\lim\limits_{ h \to 0 } \frac{1}{h}\cdot \frac{-h^{5}}{h^{4}}=-1
$$

Но $f''_{yx}(0,0)=1\neq f''_{yx}(0,0)$