$\lim\limits_{ n \to +\infty} a_{n} = a \implies \lim\limits_{ n \to +\infty} (1+\frac{a_{n}}{n})^{n} = \exp(a)$

# Следствие
* $\exp(a)\exp(b) = \exp(a+b)$
> [!info]- Док-во
> $$
> \left( 1+\frac{a}{n} \right)^{n}\left( 1+\frac{b}{n} \right)^{n} = \left( 1+\frac{a}{n} + \frac{b}{n}+\frac{ab}{n^{2}} \right)^{n}=\left( 1+\frac{ a+b+\frac{ab}{n}}{n} \right)^{n}
> $$
> $$
> \left( a+b+\frac{ab}{n} \right)\to a+b
> $$
> $$
> \left( 1+\frac{a}{n} \right)^{n}\left( 1+\frac{b}{n} \right)^{n}=\left( 1+\frac{a+b}{n} \right)^{n}
> $$
> $$
> \exp(a)\exp(b) = \exp(a+b)
> $$
* $\exp(n) = e^{n}, n \in \mathbb{N}$
* $f(x) = \exp(x)$ строг. возрастает
> [!info]- Док-во
> $t>0: \exp(x+t)=\exp(x)\exp(t)\geq (1+t)\exp(x) \geq \exp(x)$
# Док-во

$A = 1 + \frac{a}{n};\quad B = 1+\frac{a_{n}}{n}$

$$
a_{n} - \text{огр} \implies \exists M: \begin{cases}
|A| \leq 1+\frac{M}{n}\\
|B| \leq 1+\frac{M}{n}
\end{cases}
$$
Докажем, что
$$
\begin{cases}
A^{n}-B^{n} \to 0\\
\lim\limits_{ n \to +\infty} A^{n} = \exp(a) 
\end{cases} \Leftrightarrow \lim\limits_{ n \to +\infty} B^{n} =\exp(a) 
$$
$$
\begin{array}{c}
0 \leq |A^{n}-B^{n}| = |(A-B)(A^{n-1}+A^{n-2}B + \dots + AB^{n-2}+B^{n-1})| =\\
= |A-B|\cdot |A^{n-1}+A^{n-2}B + \dots + AB^{n-2}+B^{n-1}|\leq\\
\leq |A-B|\cdot(|A^{n-1}|+|A^{n-2}B|+\dots+|B^{n-1}|)\leq\\
\leq |A-B|\cdot n\left( 1+\frac{M}{n} \right)^{n-1}=\\
=|1+\frac{a}{n}-1-\frac{a_{n}}{n}|\cdot n\left( 1+\frac{M}{n} \right)^{n-1}=\\
=\frac{|a-a_{n}|}{n}\cdot n \cdot\left( 1+\frac{M}{n} \right)^{n-1} =\\
= |a-a_{n}|\left( 1+\frac{M}{n} \right)^{n-1} -\text{б/м}
\end{array}
$$
