$y_{n}$ — строг. возр. и $\lim\limits_{ n \to +\infty} y_n=+\infty$

Если $\exists \lim\limits_{ n \to +\infty} \frac{x_{n}-x_{n-1}}{y_{n}-y_{n-1}} = l \in \mathbb{\bar{R}}$, то $\lim\limits_{ n \to +\infty} \frac{x_n}{y_{n}}=l$

# Док-во

$z_{n} = \frac{x_{n}-x_{n-1}}{y_{n}-y_{n-1}}$

## Случай 1
$$
z_{n}\text{ — б/м} \Leftrightarrow \forall \varepsilon >0\ \exists N\ \forall n\geq N: |z_{n}|<\varepsilon
$$

fix $\varepsilon>0 \to N$

Выберем $N\leq m < n$
$$
x_{n}-x_{m} = (x_{n}-x_{n-1})+(x_{n-1}-x_{n-2})+(x_{n-2}-x_{n-3})+\dots+(x_{m+1}-x_{m}) = 
$$
Заметим, что $x_{n} - x_{n-1} = z_{n}(y_{n}-y_{n-1})$
$$
= z_{n}(y_{n}-y_{n-1})+\dots+z_{m+1}(y_{m+1}-y_{m})
$$
$$
\begin{gathered}
|x_{n}-x_{m}|=|\sum\limits_{k=m+1}^{n}z_{k}(y_{k}-y_{k-1})|\leq \sum\limits_{k=m+1}^{n} |z_{k}|\cdot|y_{k}-y_{k-1}| < \varepsilon \cdot \sum\limits_{k=m+1}^{n} |y_{k}-y_{k-1}| = \\
=\varepsilon \cdot \sum\limits_{k=m+1}^{n} (y_{k}-y_{k-1}) = \varepsilon\cdot(y_{n}-y_{m})
\end{gathered}
$$
$$
\begin{array}{c}
|x_{n}-x_{m}|<\varepsilon\cdot(y_{n}-y_{m})\\
|x_{n}|-|x_{m}|\leq |x_{n}-x_{m}|<\varepsilon\cdot(y_{n}-y_{m})\\
|x_{n}| < |x_{m}| + \varepsilon\cdot y_{n}\quad | :y_{n},\ y_{n}>0\\
\left|\frac{x_{n}}{y_{n}}\right| < \varepsilon + \left|\frac{x_{m}}{y_{n}}\right|
\end{array}
$$
fix $m,\ n\to +\infty$
$$
\begin{array}{c}
\left|\frac{x_{m}}{y_{n}}\right| < \varepsilon\\
\left|\frac{x_{n}}{y_{n}}\right|<2\varepsilon
\end{array}
$$
$$
\lim\limits_{ n \to +\infty} \frac{x_n}{y_{n}} = 0 
$$
**чтд**

## Случай 2

$l \in \mathbb{R},\ l\ne0$

$\widetilde{x}_{n} = x_{n} - y_{n} \cdot l$

$$
\frac{\widetilde{x}_{n} - \widetilde{x}_{n-1}}{y_{n}-y_{n-1}} = \frac{(x_{n}-y_{n}\cdot l)-x_{n-1}-y_{n-1}\cdot l}{y_{n}-y_{n-1}} = \frac{x_{n}-x_{n-1}}{y_{n}-y_{n-1}}-l \stackrel{n\to +\infty}{\to} 0 \implies \lim\limits_{ n \to +\infty} \frac{\widetilde{x}_{n}}{y_{n}}=0 
$$
$$
\frac{\widetilde{x}_{n}}{y_{n}}(\to0) = \frac{x_{n}}{y_{n}}-l \implies \lim\limits_{ n \to +\infty} \frac{x_n}{y_{n}}=l 
$$
## Случай 3

$l = +\infty$

$$
\begin{gathered}
\lim\limits_{ n \to +\infty} \frac{x_{n}-x_{n-1}}{y_{n}-y_{n-1}}=+\infty \implies \lim\limits_{ n \to +\infty} \frac{y_{n}-y_{n-1}}{x_{n}-x_{n-1}} = 0 \stackrel{1}\implies\\
\stackrel{1}\implies \lim\limits_{ n \to +\infty} \frac{y_{n}}{x_{n}}=0 \implies \lim\limits_{ n \to +\infty} \frac{x_n}{y_{n}}=+\infty    
\end{gathered}
$$

Но для $\stackrel1\implies$ нужно:

1. $x_{n}$ строго возр.
2. $x_{n} \to +\infty$

$$
\begin{gathered}
\frac{x_{n}-x_{n-1}}{y_{n}-y_{n-1}} \to +\infty \implies \text{НСНМ } \frac{x_{n}-x_{n-1}}{y_{n}-y_{n-1}} > 1 \stackrel{y_{n}-y_{n-1}>0}\implies\\
\stackrel{y_{n}-y_{n-1}>0}\implies x_{n}-x_{n-1}>0 \implies x_{n} >x_{n-1} \text{ НСНМ} 
\end{gathered}
$$

$\exists N;\ Let\ N \leq m < n$

$$
\begin{gathered}
x_{n}-x_{m} = (x_{n}-x_{n-1})+(x_{n-1}-x_{n-2})+\dots+(x_{m+1}-x_{m}) >\\
> (y_{n}-y_{n-1})+\dots+(y_{m+1}-y_{m}) = y_{n}-y_{m}
\end{gathered}
$$
$$
x_{n} - x_{m} > y_{n} - y_{m} > y_{n}
$$
fix $m,\ n\to +\infty$

$$
x_{n}>x_{m}+y_{n} \implies x_{n} \to +\infty
$$

**чтд**

## Случай 4

$l = -\infty,\ \widetilde{x}_{n}=-x_{n}$. По 3 $\frac{\widetilde{x}_{n}-\widetilde{x}_{n-1}}{y_{n}-y_{n-1}}\to+\infty$
