$0<y_{n}<y_{n-1} \forall n \in \mathbb{N}$

$\lim\limits_{ n \to +\infty} x_n=\lim\limits_{ n \to +\infty} y_{n}=0$

Если $\lim\limits_{ n \to +\infty} \frac{x_n-x_{n-1}}{y_{n}-y_{n-1}}=l\in \bar{R}$, то $\lim\limits_{ n \to +\infty} \frac{x_n}{y_{n}} =l$

## Док-во

$z_{n} = \frac{x_{n}-x_{n-1}}{y_{n}-y_{n-1}}$

### Случай 1

$l=0 \implies \forall \varepsilon>0\ \exists N\ \forall n\geq N: |z_{n}|<\varepsilon$

$N \leq m < n$

$$
x_{n}-x_{m} = (x_{n}-x_{n-1})+\dots+(x_{m+1}-x_{m}) =z_{n}(y_{n}-y_{n-1})+\dots+z_{m+1}(y_{m+1}-y_{m}) 
$$

$$
\begin{gathered}
|x_{n}-x_{m}|\leq \sum\limits_{k=m+1}^{n} |z_{k}|\cdot|y_{k}-y_{k-1}| \leq \varepsilon \cdot \sum\limits_{k=m+1}^{n} |y_{k}-y_{k-1}| =\\
=\varepsilon\cdot \sum\limits_{k=m+1}^{n}(y_{k-1}-y_{k}) = \varepsilon(y_{m}-y_{n})
\end{gathered}
$$
$$
|x_{n}-x_{m}| \leq \varepsilon(y_{m}-y_{n})
$$
при $n\to+\infty$

$$
\begin{array}{c}
|x_{m}|\leq \varepsilon \cdot y_{m}\\
\left| \frac{x_{m}}{y_{m}} \right| \leq \varepsilon\\
\lim\limits_{ n \to +\infty} \frac{x_m}{y_{m}} = 0 
\end{array}
$$

**чтд**