1. $(m, n)=1 \implies \mathbb{Z}/mn\mathbb{Z} \cong \mathbb{Z} /m\mathbb{Z} \times \mathbb{Z} / n\mathbb{Z}$
2. $m_{1}, m_{2}, \dots, m_{k}\in \mathbb{Z},\ (m_{i},m_{j})=1 \implies \mathbb{Z} / m_{1}\dots m_{k} \cong \mathbb{Z} /m_{1}\mathbb{Z} \times\dots \mathbb{Z} / m_{k}\mathbb{Z}$
3. $\forall a_{1}, \dots, a_{n} \in \mathbb{Z};\ m_{1},\dots,m_{n}\in \mathbb{Z};\ (m_{i},m_{j})=1$
	система $\begin{cases}x\equiv a_{1}\pmod{m_{1}}\\\dots\\x\equiv a_{n}\pmod{m_{n}}\end{cases}\ \exists!$ решение по $\pmod{m_{1}m_{2}\dots m_{n}} \implies$ $\implies\forall x = x_{0}+km_{1}\dots m_{n}$ 
## Док-во
### Пункт 2

Индукция по $k$

**База**: $k=2$

Строим $\phi: \mathbb{Z} /mn\mathbb{Z} \to \mathbb{Z}/m\mathbb{Z} \times \mathbb{Z} /n\mathbb{Z}$

$\overline{a}_{mn} \mapsto (\overline{a}_{m}, \overline{a}_{n})$

$\phi$ — гомоморфизм:
$$
\begin{gathered}
\phi(x+y)=\phi(\overline{a}_{mn}+\overline{b}_{mn})=\phi(\overline{a+b}_{mn} )=(\overline{a+b}_{m}, \overline{a+b}_{mn}) =\\
= (\overline{a}_{m}, \overline{a}_{n})+(\overline{b}_{m}, \overline{b}_{n}) = \phi(x)+\phi(y)
\end{gathered}
$$

Аналогично с умножением. 

$\phi$ – биекция (см [[Утверждение около КТО|утв.]])

**Переход**: $k\to k+1$

$m_{1}, \dots, m_{k+1};\ (m_{i},m_{j})=1 \implies (m_{1}\cdot \dots m_{k}, m_{k+1}) = 1$ по базе $\mathbb{Z} /m_{1}\dots m_{k+1}\mathbb{Z} \cong \mathbb{Z} /m_{1}\dots m_{k}\mathbb{Z} \times \mathbb{Z} /m_{k+1}\mathbb{Z}$

По предп. $\mathbb{Z} /m_{1}\dots m_{k}\mathbb{Z} \cong \mathbb{Z} /m_{1}\mathbb{Z} \times\dots \times \mathbb{Z} /m_{k}\mathbb{Z}$ 

Итого $\mathbb{Z}/m_{1}\dots m_{k+1}\mathbb{Z} \cong \mathbb{Z} /m_{1}\mathbb{Z} \times\dots \times \mathbb{Z} /m_{k+1}\mathbb{Z}$

>[!note]- $(A\times B)\times C\cong A\times B\times C$
>$((a, b),c)\mapsto(a,b,c)$

### Пункт 3

$\phi$ — сюръект., т.е. $\forall y_{1},\dots y_{n};\ y_{i}\in \mathbb{Z} /m_{i}\mathbb{Z}: \exists z \in \mathbb{Z} /m_{1}\dots m_{n}\mathbb{Z}: \phi(z)=(y_{1}, y_{2}, \dots, y_{n})$

Возьмём $y_{i} = \overline{a}_{i},\ a_{i}\in \mathbb{Z}$
$$
z = \overline{x}_{m_{1}\dots m_{n}} \implies \begin{cases}
\overline{x}_{m_{1}}= y_{1}\\\dots\\
\overline{x}_{m_{n}} =y_{n}
\end{cases}
$$
т.е. $\begin{cases}x\equiv a_{1}\pmod{m_{1}}\\\dots\\x\equiv a_{n}\pmod{m_{n}}\end{cases}$

Ед-ть $x$ следует из инъективности $\phi$ (по $\pmod{m_{1}\dots m_{n}}$)