Найдём $\phi ^{-1}(1_{m_{1}},0_{m_{2}}\dots, 0_{m_{k}})=a$

$$
a: \begin{cases}a-1\;\vdots\;m_{1}\\ a\;\vdots\;m_{2}\dots m_{k}\end{cases} \Leftrightarrow a=m_{2}\dots m_{k}\cdot y \implies \begin{gathered}
m_{2}\dots m_{k}\cdot y - 1=m_{1}\cdot x\\
m_{2}\dots m_{k}\cdot y -m_{1}\cdot x=1
\end{gathered}
$$
Такое ур-е мы умеем решать. 

$a = a_{1}\quad \phi(\overline{a}_{1})=(1, 0, \dots, 0)$

Аналогично находим $a_{i}: \phi(a_{i})=(0, 0\dots, \stackrel{i}1, 0, \dots , 0)$

Теперь $\forall \overline{b}_{1}\in \mathbb{Z} / m_{1}\mathbb{Z}, \dots \overline{b}_{k} \in \mathbb{Z} /m_{k}\mathbb{Z}:$
$$
\phi(\overline{a_{1}b_{1}}+\dots+\overline{a_{k}b_{k}})=\phi(b_{1}a_{1})+\dots+\phi(b_{k}a_{k}) = b_{1}\phi(a_{1})+\dots+b_{k}\phi(a_{k}) = (\overline{b}_{1}, \dots, \overline{b}_{k})
$$
