$f:D\to \mathbb{R}^{m},\ g:E\to \mathbb{R}^{l},\ f(D)\subset E\subset \mathbb{R}^{m},\ D\subset \mathbb{R}^{n},\ a \in \mathrm{Int}\,D,\ f(a) \in \mathrm{Int}\,E,\ f$ [[Дифференцируемость ФМП|дифф.]] в т. $a$, $g$ дифф. в т. $f(a)$

Тогда $(g\circ f)$ дифф. в т. $a$ и 
$$
\begin{gathered}
d_{a}(g\circ f)=d_{f(a)}g\circ d_{a}f\\
(g\circ f)'(a)=g'(f(a))\cdot f'(a)
\end{gathered}
$$
(см. [[Дифференциал ФМП]])
## Док-во

$b:=f(a)$

$$
\begin{gathered}
f(a+h)=f(a)+d_{a}f(h)+\alpha(h)\lVert h \rVert ,\ \alpha(h)\stackrel{h \to 0}\to 0\\
g(b+k)=g(b)+d_{b}g(k)+\beta(k)\lVert k \rVert,\ \beta(k)\stackrel{k\to 0}{\to}0 
\end{gathered}
$$

Возьмём $k=d_{a}f(h)+\alpha(h)\lVert h \rVert\stackrel{h\to 0}\to 0$, $f(a+h)=b+k$
$$
\begin{gathered}
g(f(a+h))=g(b+k)=g(b)+d_{b}g(k)+\beta(k)\lVert k \rVert=\\=g(f(a))+\underbrace{ d_{b}g(d_{a}f(h)) }_{ \text{лин. отобр.} }+\underbrace{ \lVert h \rVert d_{b}f(\alpha(h))+\beta(k)\cdot\lVert k \rVert  }_{ =O(\lVert h \rVert ) } 
\end{gathered}
$$
$$
d_{b}f(\alpha(h))\stackrel{h\to 0}{\to}d_{b}f(0)=0 \implies \lVert h \rVert d_{b}f(\alpha(h))=o(\lVert h \rVert )
$$
$$
\frac{\beta(k)\lVert k \rVert}{\lVert h \rVert }\stackrel{?}{\to} 0
$$
$$
\lVert k \rVert =\lVert d_{a}f(h)+\alpha(h)\lVert h \rVert  \rVert \leq \lVert d_{a}f(h) \rVert +\lVert h \rVert \cdot \lVert \alpha(h) \rVert \leq \lVert d_{a}f \rVert \cdot \lVert h \rVert +\underbrace{ \lVert \alpha(h) \rVert }_{ \to 0\implies \text{огр.} } \cdot \lVert h \rVert 
$$