$W_{n} = \int\limits_{0}^{\pi/2}\cos ^{n}x\,dx\stackrel{(*)}{=}\int\limits_{0}^{\pi/2}\sin ^{n}x\,dx$

>[!note]- Пояснение к (\*)
> $$
> \int\limits_{0}^{\pi/2} \sin ^{n}x\,dx=\int\limits_{0}^{\pi/2} \cos ^{n}\left( \frac{\pi}{2}-t \right)\,dt=-\int\limits_{\phi(0)=\frac{\pi}{2}}^{\phi(\pi/2)=0} \cos ^{n}x\,dx=\int\limits_{0}^{\pi/2}\cos ^{n}\,dx 
> $$

$W_{0}=\frac{\pi}{2}$
$W_{1}=\int\limits_{0}^{\pi/2}\sin x\,dx=-\cos x\bigg|_{0}^{\pi/2}=1$
$W_{2}=\frac{1}{2}\left( \int\limits_{0}^{\pi/2}\cos ^{2}x+\int\limits_{0}^{\pi/2}\sin ^{2}x \right)=\frac{\pi}{4}$
$$
\begin{gathered}
W_{n}=\int\limits_{0}^{\pi/2} \sin ^{n}x\,dx=\int\limits_{0}^{\pi/2} \sin ^{n-1}x(-\cos x)'\,dx
=\left[ \begin{gathered}
u=\sin ^{n-1}x\\ v=-\cos x\\ u'=(n-1)\sin ^{n-2}x\cos x
\end{gathered} \right] =\\=\underbrace{ \sin ^{n-1}x(-\cos x)\bigg|_{0}^{\pi/2} }_{ 0 }-\int\limits_{0}^{\pi/2} (n-1)\sin ^{n-2}x\cos x(-\cos x)\,dx=\\
=(n-1)\int\limits_{0}^{\pi/2} \sin ^{n-2}x(1-\sin ^{2}x)\,dx=\\
=(n-1)\left( \int\limits_{0}^{\pi/2} \sin ^{n-2}x\,dx-\int\limits_{0}^{\pi/2} \sin ^{n}x\,dx \right)=(n-1)(W_{n-2}-W_{n})\implies\\
\implies nW_{n}=(n-1)W_{n-2}
\end{gathered}
$$

Тогда выражение зависит от чётности:
$$
\begin{gathered}
W_{2n}=\frac{2n-1}{2n}W_{2n-2}=\frac{2n-1}{2n}\cdot \frac{2n-3}{2n-2}W_{2n-4}=\dots =\\
= \frac{(2n-1)(2n-3)\dots1}{2n(2n-2)\dots 2}\cdot \frac{\pi}{2}=\frac{(2n-1)!!}{2n!!}\cdot \frac{\pi}{2}
\end{gathered}
$$
$$
\begin{gathered}
W_{2n+1}= \frac{2n}{2n+1}W_{2n-1}= \frac{2n}{2n+1} \cdot \frac{2n-2}{2n-1}W_{2n-3}=\dots=\\
= \frac{2n(2n-2)\dots 2}{(2n+1)(2n-1)\dots 3} = \frac{(2n)!!}{(2n+1)!!}
\end{gathered}
$$
