$H_{j}:= \frac{1}{j!}\int\limits_{0}^{\pi/2}\left( \left( \frac{\pi}{2} \right)^{2}-x^{2} \right)^{j}\cos x\,dx$
## Свойства

1. $0<H_{j}\leq \frac{1}{j!}\int\limits_{0}^{\pi/2}\left( \frac{\pi}{2} \right)^{2j}\cos x\,dx=\frac{ \left( \frac{\pi}{2} \right)^{2j}}{j!}$
2. Если $c>0$: $c^{j}H_{j}\stackrel{j\to \infty}{\to}0$
>[!note]- Док-во
>$0<c^{j}H_{j}\leq \frac{\left( c\cdot \frac{\pi^{2}}{4} \right)^{j}}{j!}\to 0$ ^366c44
3. $H_{0}=1,\ H_{1}=2$
4. при $j\geq 2: H_{j}=(4j-2)H_{j-1}-\pi^{2}H_{j-2}$
5. Существует мн-н $P_{j}$ степени $\leq j$ с целыми коэф., т.ч. $H_{j}=P_{j}(\pi^{2})$
>[!note]- Док-во
> $P_{0} \equiv 1,\ P_{1}\equiv 2$
> $$
> \begin{gathered}
> P_{j}(x)=(4j-2)P_{j-1}-xP_{j-2}(x)\implies P_{j}(\pi^{2})=(4j-2)\underbrace{ P_{j-1}(\pi^{2}) }_{ H_{j-1} }-\pi^{2}\underbrace{ P_{j-2}(\pi^{2}) }_{ H_{j-2} }
> \end{gathered}
> $$
