$f \in C^{n+1}\langle a,b \rangle,\ x_{0},x \in \langle a, b \rangle$.

Тогда 
$$
f(x)=\sum\limits_{k=0}^{n} \frac{f^{(k)}(x_{0})}{k!}(x-x_{0})^{k}+\frac{1}{n!}\int\limits_{x_{0}}^{x} (x-t)^{n}f^{(n+1)}(t)\,dt
$$
## Док-во

(ММИ по $n$).

**База**: $n=0$:
$$
f(x)=f(x_{0})+\frac{1}{0!}\underbrace{ \int\limits_{x_{0}}^{x} f'(t)\,dtU }_{ \text{Ньютон-Лейбниц } f(x)-f(x_{0}) } 
$$
**Переход**: $n\to n+1$
$$
\begin{gathered}
f(x)=\sum\limits ^{n}_{k=0} \frac{f^{(k)}(x_{0})}{k!}(x-x_{0})^{k}+\frac{1}{n!}\int\limits_{x_{0}}^{x} (x-t)^{n}f^{(n+1)}(t)\,dt=\\
=\sum\limits ^{n}_{k=0} \frac{f^{(k)}(x_{0})}{k!}(x-x_{0})^{k}+\int\limits_{x_{0}}^{x} (x-t)^{n}f^{(n+1)}(t)\,dt=\left[ \begin{gathered}
u=f^{(n+1)}\\ v'=(x-t)^{n}\\ v= -\frac{(x-t)^{n+1}}{n+1}
\end{gathered} \right] =\\
=\underbrace{ -f^{(n+1)}(t) \frac{(x-t)^{n+1}}{n+1}\bigg|_{t=x_{0}}^{t=x} }_{ =f^{(n+1)}(x_{0}) \frac{(x-xo_{0})^{n+1}}{n+1} }+\int\limits_{x_{0}}^{x} \frac{(x-t)^{n+1}}{n+1}f^{(n+2)}(t)\,dt 
\end{gathered}
$$