$a_{k}, b_{k}\geq 0;\ \frac{1}{p}+\frac{1}{q}=1;\ q,p>1$

Тогда 
$$
\sum\limits_{k=1}^{n}a_{k}b_{k}\leq \left( \sum\limits a_{k}^{p} \right)^{1/p}\cdot \left( \sum\limits b_{k}^{q} \right)^{1/q}
$$
## Док-во

$B:= \left( \sum\limits_{k=1}^{n}b_{k}^{q} \right)^{1/q}$

Будем считать, что $B>0$

Заметим, что наше нер-во равносильно:
$$
\sum\limits_{k=1}^{n}a_{k}\cdot \frac{b_{k}}{B}\leq \left( \sum\limits_{k=1}^{n} a_{k}^{p} \right)^{1/p}\Leftrightarrow \left( \sum\limits a_{k}\cdot \frac{b_{k}}{B} \right)^{p}\leq \sum\limits_{k=1}^{n}a_{k}^{p}
$$
$f(x)=x^{p}\implies f(x)$ — выпукл ($p>1$). Тогда
$$
\sum\limits(\lambda_{k}x_{k})^{p}\leq \sum\limits \lambda_{k}x_{k}^{p}
$$
Хотим:
$$
\frac{\cdot}{\cdot}
\begin{cases}
\lambda_{k}x_{k}=a_{k} \cdot \frac{b_{k}}{B}\\
\lambda_{k}x_{k}^{p}=a_{k}^{p}
\end{cases}\implies x_{k}^{p-1}= \frac{a_{k}^{p-1}\cdot B}{b_{k}};\ x_{k}= \frac{a_{k}B^{1/(p-1)}}{b_{k}^{1/(p-1)}}
$$
$$
\begin{gathered}
\frac{1}{p}+\frac{1}{q} = 1\implies \frac{1}{q}=1-\frac{1}{p}=\frac{p-1}{p}\implies q = \frac{p}{p-1}\implies\\\implies x_{k}^{p} = \frac{a_{k}^{p}B^{p/(p-1)}}{b_{k}^{q}} \implies \lambda_{k} = \frac{b_{k}^{q}}{B^{q}}
\end{gathered}
$$
