$p\geq 1;\ a_{k},b_{k}\geq0$

Тогда 
$$
\left( \sum\limits(a_{k}+b_{k})^{p} \right)^{1/p}\leq \left( \sum\limits a_{k}^{p} \right)^{1/p}+\left( \sum\limits b_{k}^{p} \right)^{1/p}
$$
## Док-во

$p>1 \implies \exists q>1: \frac{1}{p}+\frac{1}{q}=1\Leftrightarrow p+q=pq$

$$
\sum\limits (a_{k}+b_{k})^{p} = \sum\limits a_{k}(a_{k}+b_{k})^{p-1}+\sum\limits b_{k}(a_{k}+b_{k})^{p-1}
$$
$$
\begin{gathered}
\sum\limits a_{k}(a_{k}+b_{k})^{p-1}\stackrel{\text{Гёльдер}}{\leq} \left( \sum\limits(a_{k}^{p}) \right)^{1/p}\cdot \left( \sum\limits(a_{k}+b_{k})^{q(p-1)} \right)^{1/q}=\\=\left( \sum\limits a_{k}^{p} \right)^{p}\left( \sum\limits(a_{k}+b_{k})^{p} \right)^{1/q}
\end{gathered}
$$
>[!note] $(p-1)q = pq-q = p$

$$\begin{gathered}
\sum\limits(a_{k}+b_{k})^{p}\leq \left( \sum\limits a_{k}^{p} \right)^{1/p}\left( \sum\limits(a_{k}+b_{k})^{p} \right)^{1/q}+\left( \sum\limits b_{k}^{p} \right)^{1/p}\left( \sum\limits(a_{k}+b_{k})^{p} \right)^{1/q}=\\
=\left( \sum\limits(a_{k}+b_{k})^{p} \right)^{1/q}\left( \left( \sum\limits a_{k}^{p} \right)^{1/p}+\left( \sum\limits b_{k}^{p} \right)^{1/p} \right)\quad\text{(поделим)}\\[10pt]
\left( \sum\limits(a_{k}+b_{k})^{p} \right)^{1/p} \leq \left( \sum\limits a_{k}^{p} \right)^{1/p}+\left( \sum\limits b_{k}^{p} \right)^{1/p} 
\end{gathered}
$$