$f: \langle a,b \rangle\to \mathbb{R};\ f$ непр и стр монот

$m=\inf_{x \in \langle a,b \rangle}f(x),\ M  =\sup_{x \in \langle a,b \rangle};\ m,M\in \mathbb{R}$

1. $f$ обр и $f^{-1}: \langle m,M \rangle\to \langle a,b \rangle$
2. $f^{-1}$ стр монот (хар-тер монот сохраняется)
3. $f^{-1}$ непр на $\langle m, M \rangle$
# Док-во
## Пункт 1

$f$ стр монот $\implies f$ инъект $\implies$ обратима
## Пункт 2

НУО $f(x)$ стр возрастает ($x>y \Leftrightarrow f(x)>f(y)$)

$f^{-1}:\langle m, M \rangle\to \langle a,b \rangle$

$u>v \stackrel{?}{\implies} f^{-1}(u)>f^{-1}(v)$

$\exists x, y: \underbrace{ f(x) }_{ =u }>\underbrace{ f(y) }_{ =v }\stackrel{1}{\implies} f^{-1}(f(x))>f^{-1}(f(y))$
## Пункт 3

$y_{0}\in \langle m,M \rangle$

Хочу док-ть, что $f^{-1}$ непр в т. $y_{0}$

$\lim\limits_{ y \to y_{0} }f^{-1}(x)=f^{-1}(y_{0})$
 
$$
\begin{gathered}
\text{на }\langle m, y_{0})\ f^{-1}\text{ возр }\implies f^{-1}(y_{0})\geq f^{-1}(y)\ \forall y \in \langle m,y_{0}) \implies\\
\implies\exists \lim\limits_{ y \to y_{0-} }f^{-1}(y)=\sup_{\langle m,y_{0})}f^{-1}(y)\leq f^{-1}(y_{0})
\end{gathered}
$$
$$
\begin{gathered}
\text{на }(y_{0},M \rangle \ f^{-1}\text{ возр }\implies f^{-1}(y)\geq f^{-1}(y_{0})\ \forall y \in (y_{0},M \rangle \implies\\
\implies\exists \lim\limits_{ y \to y_{0+} }f^{-1}(y)=\inf_{(y_{0},M \rangle}f^{-1}(y)\geq f^{-1}(y_{0})
\end{gathered}
$$

$$
\lim\limits_{ y \to y_{0}+ } f^{-1}(y)=A\leq f^{-1}(y_{0})\leq B=\lim\limits_{ y \to y_{0}- } f^{-1}(y)
$$

* если $A=B$ — доказано

Что знаем: $A\leq B$

Пусть $A<B$

$f^{-1}:\langle m,M \rangle\to \langle a,b \rangle$

$f^{-1}(\langle m,M \rangle)=\langle a,b \rangle$

$$
\begin{gathered}
\langle m,M \rangle \subset (-\infty;A]\cup \{ f^{-1}(y_{0}) \}\cup [B;+\infty) \implies A=B \implies\\
\implies\lim\limits_{ y \to y_{0}+ } f^{-1}(y)=\lim\limits_{ y \to y_{0}- } f^{-1}(y)=f^{-1}(y_{0}) \implies \lim\limits_{ y \to y_{0} } f^{-1}(y)=f^{-1}(y_{0})
\end{gathered}
$$