$\phi(n) = |(\mathbb{Z} /n\mathbb{Z})^{*}|$

$\phi(n)= |\{ x \in \{ 0, \dots, n-1 \}: (x,n)=1 \}|$

## Как найти $\phi(n)$

### Для $p \in \mathbb{P}$
$\phi(p^{k})=|\{ x=0\dots p^{k}-1:(p^{k}, x)=1 \}|=p^{k}-\{ x=0\dots p^{k}-1: x \;\vdots\; p \}=p^{k}-\frac{p^{k}}{p}=p^{k}-p^{k-1}$
### Мультипликативность $\phi$

$$
\begin{gathered}
m, n \in \mathbb{N}\\
(m, n)=1
\end{gathered}\implies \phi(m\cdot n)=\phi(m)\cdot \phi(n)
$$

#### Док-во

Знаем, что $(m, n)=1 \implies \mathbb{Z} /mn\mathbb{Z} \cong \mathbb{Z} /n\mathbb{Z} \times \mathbb{Z} /m\mathbb{Z}$

Пусть $f: \mathbb{Z} / mn\mathbb{Z} \to \mathbb{Z} /n\mathbb{Z} \times \mathbb{Z} /m\mathbb{Z}$ — изоморфизм.

Тогда $x$ — обратим $\Leftrightarrow f(x)$ — обратим. 

**Следствие**: $(\mathbb{Z} /nm\mathbb{Z})* = (\mathbb{Z} /n\mathbb{Z} \times \mathbb{Z} /m\mathbb{Z})*$

> [!info]- **Утв-е**: $R_{1}, R_{2}$ — кольца. $(R_{1}\times R_{2})* = R_{1}* \times R_{2}*$
> $(r_{1}, r_{2}) \in R_{1}\times R_{2}$ — обратим
> $$
> \begin{gathered}
> \Leftrightarrow \exists (s_{1}, s_{2}): (r_{1}, r_{2})\cdot(s_{1}, s_{2}) = 1_{R_{1}\times R_{2}}\\
> \Leftrightarrow (r_{1}s_{1}, r_{2}s_{2})=(1_{R_{1}}, 1_{R_{2}})\\
> \Leftrightarrow \exists s_{1}, s_{2}: \begin{cases}
> r_{1}s_{1}=1_{R_{1}}\\
> r_{2}s_{2}=1_{R_{2}}
> \end{cases}
> \end{gathered}
> $$

**Сл-е**: $|(\mathbb{Z} /nm\mathbb{Z})*| = |(\mathbb{Z} /n\mathbb{Z} \times \mathbb{Z} /m\mathbb{Z})*| \implies \phi (mn) = \phi(n)\phi(m)$ при $(m, n)=1$

**чтд**

### Явная формула
$$
\begin{gathered}
\phi(n)=\phi(p_{1}^{a_{1}}\dots p_{k}^{a_{k}})=\phi(p_{1}^{k_{1}})\cdot \phi(p_{2}^{a_{2}}\dots p_{k}^{a_{k}}) = \phi(p_{1}^{a_{1}})\dots \phi(p_{k}^{a_{k}})=\\
=(p_{1}^{a_{1}}-p_{1}^{a_{1}-1})\dots(p_{k}^{a_{k}}-p_{k}^{a_{k}-1})=p_{1}\left( 1-\frac{1}{p_{1}} \right)\dots p_{k}\left( 1-\frac{1}{p_{k}} \right) =\\
= n\left( 1-\frac{1}{p_{1}} \right)\dots\left( 1-\frac{1}{p_{k}} \right)
\end{gathered}
$$
