$f,g: \langle a,b \rangle\to \mathbb{R};\ x_{0} \in \langle a,b \rangle$
$f$ и $g$ $n$ раз дифф в т. $x_{0}$

Тогда
1. $\alpha,\beta \in \mathbb{R}: \alpha f+\beta g$ — $n$ раз дифф в т. $x_{0}$ и $(\alpha f+\beta g)^{(n)}(x_{0})=\alpha f^{(n)}(x_{0})+\beta g^{(n)}(x_{0})$
2. $fg$ — $n$ раз дифф в т. $x_{0}$ и $(fg)^{(n)}(x_{0})=\sum\limits ^{n}_{k=0}{n\choose k}f^{(k)}(x_{0})g^{(n-k)}(x_{0})$ (**ф-ла Лейбница**)
3. $f(\alpha x+\beta)$ — $n$ дифф в т. $x_{0}$ и $(f(\alpha x+\beta))^{(n)}(x_{0})=\alpha^{n}f^{(n)}(\alpha x_{0}+\beta)$
# Примеры
1. $(x^{p})^{(n)}=p(p-1)\dots(p-n+1)x^{p-n}$
2. $\left( \frac{1}{x} \right)^{(n)}=(-1)(-2)\dots(-n)\cdot \frac{1}{x^{n+1}}= \frac{(-1)^{n}n!}{x^{n+1}}$
3. $(\ln x)^{(n)}=((\ln x)')^{(n-1)}=\left( \frac{1}{x} \right)^{(n-1)}= \frac{(-1)^{n-1}(n-1)!}{x^{n}}$
4. $(a^{x})^{(n)}=(\ln a\cdot a^{x})^{(n-1)}=(\ln a)^{n}\cdot a^{x}$
5. $(\sin x)^{(n)}=\sin\left( x+\frac{\pi}{2}n \right)$
6. $(\cos x)^{(n)}=\cos\left( x+\frac{\pi}{2}\cdot n \right)$
# Док-во
## Пункт 1

База: $n=1$
Переход: $n\to n+1$
$$
\begin{gathered}
(\alpha f+\beta g)^{(n+1)}(x_{0})=((\alpha f+\beta g)^{(n)})'(x_{0})=(\alpha f^{(n)}(x)+\beta g^{(n)}(x))'(x_{0})=\\=\alpha f^{(n+1)}(x_{0})+\beta g^{(n+1)}(x_{0})
\end{gathered}
$$
## Пункт 2

База: $n=1$
$$
(fg)'(x_{0})=f'(x_{0})g(x_{0})+f(x_{0})g'(x_{0})=\sum\limits ^{1}_{k=0}{1\choose k}f^{(k)}(x_{0})g^{(1-k)}(x_{0})
$$
Переход: $n\to n+1$

$$
\begin{gathered}
(fg)^{(n+1)}(x_{0})=((fg)^{(n)})'(x_{0})=\left( \sum\limits ^{n}_{k=0}{n\choose k}f^{(k)}g^{(n-k)} \right)'(x_{0})=\sum\limits_{k=0}^{n}{n\choose k}(f^{(k)}g^{(n-k)})'=\\
=\sum\limits_{k=0}^{n}{n\choose k}(f^{(k+1)}g^{(n-k)}+f^{(k)}g^{(n-k+1)})=\\
=\sum\limits_{k=0}^{n}{n\choose k}f^{(k+1)}g^{(n-k)}+\sum\limits_{k=0}^{n}{n\choose k}f^{(k)}g^{(n+1-k)}=\\
=\sum\limits_{m=1}^{n+1}{n\choose m-1}f^{(m)}g^{(n+1-m)}+\sum\limits_{m=0}^{n} {n\choose m}f^{(m)}g^{(n+1-m)}=\\
=\sum\limits_{m=1}^{n} {n\choose m}f^{(m)}g^{(n+1-m)}+\left({n\choose m-1}+{n\choose m}\right)f^{(m)}g^{(n+1-m)}=\sum\limits_{m=0}^{n+1}{n+1\choose m}f^{(m)}g^{(n+1-m)}
\end{gathered}
$$