$f$ — $n$ раз дифф в т. $x_{0},\ P(x)$ — мн-н степ. $\leq n;\ f(x)=P(x)+o((x-x_{0})^{n})$

Тогда $P(x)=T_{n,x_{0}}f(x)$

# Док-во

$P(x)-T_{n,x_{0}}f(x)=\sum\limits_{k=0}^{n}a_{k}(x-x_{0})^{k}=o((x-x_{0})^{n})$

Пусть не все $a_{k}=0\implies a_{m}\ne 0$ — наим. ненулевой.

$P(x)-T_{n,x_{0}}=\sum\limits_{k=m}^{n}a_{k}(x-x_{0})^{k}$
$$
\begin{gathered}
\sum\limits_{k=m}^{n}a_{k}(x-x_{0})^{k}=o((x-x_{0})^{n})\quad|\cdot \frac{1}{(x-x_{0})^{m}}\\
\begin{cases}
\lim\limits_{ x \to x_{0} } \frac{o(x-x_{0})^{n}}{(x-x_{0})^{m}}=0\\
\lim\limits_{ x \to x_{0} } \frac{\left( \sum\limits_{k=m}^{n}a_{k}(x-x_{0})^{k} \right)}{(x-x_{0})^{m}}=a_{m}
\end{cases}
\end{gathered}
$$
получ. пр-чие.