$g(x)$ — $n$ раз д-ма в т. $x_{0}$ и $g(x_{0})=g'(x_{0})=g''(x_{0})=\dots=g^{(n)}(x_{0})=0$

Тогда $g(x)=o((x-x_{0})^{n}), x\to x_{0}$

## Док-во

$g(x)=o((x-x_{0})^{n})\Leftrightarrow \lim\limits_{ x \to x_{0} } \frac{g(x)}{(x-x_{0})^{n}}=0$

$$
\begin{gathered}
\lim\limits_{ x \to x_{0} } \frac{g(x)}{(x-x_{0})^{n}}\stackrel{Лоп.\ \left\{  \frac{0}{0}  \right\}}{=} \lim\limits_{ x \to x_{0} } \frac{g'(x)}{n(x-x_{0})^{n-1}}\stackrel{\left\{  \frac{0}{0}  \right\}}{=}\\
=\lim\limits_{ x \to x_{0} } \frac{g''(x)}{n(n-1)(x-x_{0})^{n-2}}=\dots=\lim\limits_{ x \to x_{0} } \frac{g^{(n-1)}(x)}{n!(x-x_{0})}=\\
=\lim\limits_{ x \to x_{0} } \frac{o(x-x_{0})}{n!(x-x_{0})}=0
\end{gathered}
$$
$g^{(n-1)}(x)$ дифф в т. $x_{0}\Leftrightarrow g^{(n-1)}(x)=\underbrace{ g^{(n-1)}(x_{0}) }_{ =0 }+\underbrace{ g^{(n)}(x_{0}) }_{ =0 }(x-x_{0})+o(x-x_{0})$
