$T(x)$ — многочлен степени $n$, тогда $T(x)=\sum\limits_{k=0}^{n} \frac{T^{(k)}(x_{0})}{k!}(x-x_{0})^{k}$
# Док-во
## Лемма 1

$T(x)=\sum\limits_{k=0}^{n}a_{k}x^{k}$, то его можно представить в виде $T(x)=\sum\limits_{k=0}^{n}c_{k}(x-x_{0})^{k}$
$$
T(x)=\sum\limits_{k=0}^{n}a_{k}x^{k}=\sum\limits_{k=0}^{n}a_{k}(\underbrace{ x-x_{0} }_{ t }+x_{0})^{k}=\sum\limits_{k=0}^{n}a_{k}(t+x_{0})^{k}=\sum\limits_{k=0}^{n}c_{k}t^{k}=\sum\limits_{k=0}^{n}c_{k}(x-x_{0})^{k}
$$
## Лемма 2
$f(x)=(x-x_{0})^{k}$, то $f^{(m)}(x_{0})=\begin{cases}m!,\ m=k\\ 0,\ m\ne k\end{cases}$

## Док-во (теоремы)

$T(x)\stackrel{\text{Lm1}}{=} \sum\limits_{k=0}^{n}c_{k}(x-x_{0})^{k}$
$T^{(m)}(x_{0})=\left( \sum\limits_{k=0}^{n}c_{k}(x-x_{0})^{k} \right)^{(m)}\biggr|_{x=x_{0}}\stackrel{Lm2}{=}c_{m}\cdot m!$
$c_{m}=\frac{T^{(m)}(x_{0})}{m!}$
$T(x)=\sum\limits_{k=0}^{n} \frac{T^{(k)}(x_{0})}{k!}(x-x_{0})^{k}$