$f:\langle a,b \rangle\to \mathbb{R}$
$f$ — $(n+1)$ раз дифф на $\langle a,b \rangle$
$x, x_{0}\in \langle a,b \rangle$

Тогда $\exists c$ м/ду $x$ и $x_{0}:$
$$
\begin{gathered}
f(x)=T_{n,x_{0}}f(x)+ \frac{f^{(n+1)}(c)}{(n+1)!}(x-x_{0})^{n+1}=\\
=\sum\limits_{k=0}^{n} \frac{f^{(k)}(x_{0})}{k!}(x-x_{0})^{k}+ \underbrace{ \frac{f^{(n+1)}(c)}{(n+1)!}(x-x_{0})^{n+1} }_{ \text{ост. в ф. Лагранжа} }
\end{gathered}
$$

# Док-во

$\pu{ fix } x \in \langle a,b \rangle$
$f(x)=T_{n,x_{0}}f(x)+M\cdot(x-x_{0})^{n+1}$

Найдём $M$, т.ч. вып-ся рав-во (хотим $M= \frac{f^{(n+1)}(c)}{(n+1)!}$)

$g(t)=f(t)-T_{n,x_{0}}f(t)-M(t-x_{0})^{n+1}$

$g(t)$ — $(n+1)$ раз дифф на $\langle a,b \rangle$

$g(x)=0;\ g(x_{0})=g'(x_{0})=g''(x_{0})=\dots=g^{(n)}(x_{0})=0$

$[x;x_{0}]$ т. Ролля для $g(t): g(x)=g(x_{0})=0\implies \exists c_{1}:g'(c_{1})=0$

$$
\begin{array}{l}
[c_{1},x_{0}]\ g'(t)\\
g'(c_{1})=g'(x_{0})=0
\end{array} \stackrel{\text{т.Ролля}}{\implies} \exists c_{2} \in [c_{1};x_{0}]: g''(c_{2})=0
$$
и тд: $\exists c \in [c_{n};x_{0}]:g^{(n+1)}(c)=0$

$g^{(n+1)}(c)=f^{(n+1)}(c)+0-M(n+1)! =0\implies M=\frac{f^{(n+1)}(c)}{(n+1)!}$