$f$ — $n$ раз дифф в т. $x_{0}$, тогда 
$$
f(x)=T_{n,x_{0}}f(x)+o((x-x_{0})^{n})=\sum\limits_{k=0}^{n} \frac{f^{(k)}(x_{0})}{k!}(x-x_{0})^{k}+o((x-x_{0})^{n}),\ x\to x_{0}
$$
## Док-во

$f(x)-T_{n,x_{0}}f(x)=g(x)$ — дифф в т. $x_{0}\ n$ раз

$$
\begin{gathered}
g^{(m\leq n)}(x_{0})=f^{(m)}(x_{0})-(T_{n,x_{0}}f(x))^{(m)}\biggr|_{x=x_{0}}=f^{(m)}(x_{0})-\frac{f^{(m)}(x_{0})}{m!}\cdot m! =0
\end{gathered}
$$
$g(x_{0})=f(x_{0})-T_{n,x_{0}}f(x_{0})=0$
$$
\forall 0\leq m \leq n:
g^{(m)}(x_{0})\stackrel{Lm}{\implies}g(x)=o((x-x_{0})^{n}),\ x\to x_{0}
$$
([[Лемма об о-малое]])
