$x_{0}=0$

1. $e^{x}=\sum\limits_{k=0}^{n} \frac{x^{k}}{k!}+o(x^{n})$
	$\forall k: f^{(k)}(0)=1$
2. $\sin x=x-\frac{x^{3}}{3!}+\frac{x^{5}}{5!}-\dots+ \frac{(-1)^{n}x^{2n+1}}{(2n+1)!}+o(x^{2n+1})$
	$(\sin x)^{(k)}=\sin\left( x+\frac{\pi}{2}k \right)\biggr|_{x=0}=\sin\left( \frac{\pi}{2}k \right)$
3. $\cos x=1-\frac{x^{2}}{2!}+\frac{x^{4}}{4!}-\dots+\frac{(-1)^{n}x^{2n}}{(2n)!}+o(x^{2n})$
	$f^{(k)}(0)=\cos\left( \frac{\pi}{2}k \right)$
4. $f(x)=\ln(1+x)=x-\frac{x^{2}}{2}+\frac{x^{3}}{3}-\frac{x^{4}}{4}+\dots+\frac{(-1)^{n-1}x^{n}}{n}+o(x^{n})$
	$f^{(k)}(x)= \frac{(-1)^{k-1}(k-1)!}{(1+x)^{k}}$
	$f^{(k)}(0)=(-1)^{k-1}(k-1)!$
5. $f(x)=(1+x)^{p}=1+px+\frac{p(p-1)}{2!}x^{2}+\frac{p(p-1)(p-2)}{3!}x^{3}+\dots+ \frac{p(p-1)\dots(p-n+1)}{n!}x^{n}+o(x^{n})$
	$((1+x)^{p})^{(k)}\biggr|_{x=0}=p(p-1)(p-k+1)(1+x)^{p-k}\biggr|_{x=0}=p(p-1)\dots(p-k+1)$
