$char(k)=0$ или $char(k)>\deg f=n$

Тогда $f=\sum\limits_{k=0}^{n} \frac{f^{(k)}(a)}{k!}(x-a)^{k}$

## Док-во

Знаем: $f=\sum\limits a_{i}(x-a)^{i}\ \mathbf{(*)}$

Хотим: $a_{i}= \frac{f^{(i)}(a)}{i!}$

Нап-е: $((x-a)^{k})'=k(x-a)^{k-1}$

Отсюда: 
$$
\begin{array}{l}
f=(x-a)^{k}\\
f^{(1)}=k(x-a)^{k-1}\\
f^{(2)}=k(k-1)(x-a)^{k-2}\\
\dots\\
f^{(k)}=k!(x-a)^{0}=k!\\
f^{(l>k)}=0
\end{array}
$$

Применим к $(*)$ дифф-е $k$ раз и эвалюируем в т. $a$.

$$
\begin{gathered}
f^{(k)}(a)=\sum\limits(a_{i}(x-a)^{i})^{(k)}=\sum\limits\begin{cases}
0\text{ при } i\ne k\\
a_{i}\cdot k!\text{ при } i=k
\end{cases}=a_{i}k! \implies\\\implies a_{i}=\frac{f^{(k)}(a)}{k!}
\end{gathered}
$$

Формально
$$
f^{(k)}(a)=a_{i}(\underbrace{ 1+\dots+1 }_{ k })(\underbrace{ 1+\dots+1 }_{ k-1 })\dots \stackrel{\text{по огр на char}}{\ne}0\implies \exists \frac{1}{k!}
$$