1. $\sim$ — отн. эквив.
	1. рефл. $f\sim f,\ x \to a$ — очев ($\phi(x)=1\ \forall x \in E$)
	2. симм. $f\sim g,\ x\to a\implies g\sim f$
	3. транз. $\begin{cases}f\sim g\\g\sim h,\ x\to a\end{cases} \implies f\sim h,\ x\to a$

> [!note]- Док-во (симм.)
> $$
> 		\begin{cases}f(x)=\phi(x)g(x),\ \mathring{U}_{a}\cap E\to \phi(x)\ne 0\\ \phi(x)\stackrel{x\to a}{\to} 1\end{cases}\implies g(x)=\underbrace{ \frac{1}{\phi(x)} }_{ \psi(x)\to 1 }f(x)\implies g\sim f
> 		$$

> [!note]- Док-во (транз.)
> $$
> f(x)=\phi(x)\cdot g(x)=\underbrace{ \phi(x)\psi(x) }_{ \to 1 }h(x)\implies f\sim h,\ x\to a
> $$

2. $\begin{array}{l}f_{1}\sim g_{1}\\ f_{2}\sim g_{2}\end{array}\implies f_{1}f_{2}\sim g_{1}g_{2},\ x\to a$
> [!note]- Док-во
> $$
> \begin{array}{l}
> f_{1}=\phi_{1}g_{1}\\f_{2}=\phi_{2}g_{2}\end{array}\implies f_{1}f_{2}=\underbrace{ \phi_{1}\phi_{2} }_{ \to1 }g_{1}g_{2} 
> $$

3. $\begin{array}{l}f_{1}\sim g_{1}\\ f_{2}\sim g_{2}\\ f_{2},\ g_{2}\ne 0\end{array}\implies \frac{f_{1}}{f_{2}}\sim \frac{g_{1}}{g_{2}}$
> [!note]- Док-во
> $$
> \frac{f_{1}}{f_{2}}=\underbrace{ \left( \frac{\phi_{1}}{\phi_{2}} \right) }_{ \to1 } \frac{g_{1}}{g_{2}}
> $$

4. $f\sim g\implies \begin{cases}f=g+o(g)\\ g=f+o(f)\end{cases}$
> [!note]- Док-во
> $$
> \begin{gathered}
> f\sim g\implies \exists \phi: f(x)=\phi(x)g(x)\implies f(x)=g(x)+\underbrace{ (\phi(x)-1) }_{ \to0 }g(x)\implies\\\stackrel{\text{def}}{\implies}f(x)=g(x)+o(g)
> \end{gathered}
> $$

5. $f\sim g\implies f=O(g)$
> [!note]- Док-во
> $$
> f(x)=\underbrace{ \phi(x) }_{ \to 1\implies \phi\text{ - огр} }g(x)\implies f=O(g)
> $$


6. $\begin{gathered}o(f)+o(f)=o(f)\\ \underbrace{ O(f) }_{ =h }+\underbrace{ O(f) }_{ =g }=O(f)\end{gathered}$

> [!note]- Док-во (1)
> $$
> \begin{cases}
> \phi(x)f(x)=o(f)\\
> \psi(x)f(x)=o(f)
> \end{cases}
> $$
> $$
> \begin{cases}
> h(x)=\phi(x)f(x),\ \phi(x)\to 0\\
> g(x)=\psi(x)f(x),\ \psi(x)\to 0
> \end{cases}\implies h(x)+g(x)=(\phi(x)+\psi(x))f(x)
> $$
> 
> Но $\phi(x)+\psi(x)\to 0\implies h(x)+g(x)\in o(f)$

> [!note]- Док-во (2)
> $$
> 		\begin{array}{l}
> 		h=\phi f\\
> 		g=\psi f;\ \psi, \phi\text{ - огр}
> 		\end{array} \implies h+g=\underbrace{ (\phi+\psi) }_{ огр }f\implies h+g=O(f)
> $$

7. $f\cdot \underbrace{ o(g) }_{ =h }=o(fg)$
> [!note]- Док-во
> $$
> \begin{array}{l}
> h=\phi g,\ \phi\to 0\\
> fh=f\phi g=\phi(fg)\implies fh=o(fg)
> \end{array} 
> $$

8. $\lim\limits_{ x \to a }f(x)=b\Leftrightarrow f(x)=b+o(1),\ x\to a$
> [!note]- Док-во
> $$
> \begin{gathered}
> \lim\limits_{ x \to a } (f(x)-b)=0\\
> \Updownarrow\\
> f(x)-b=\phi(x),\ \phi(x)\to 0\\
> f(x)=b+\underbrace{ \phi(x) }_{ o(1) },\ x\to a
> \end{gathered}
> $$