$(rz_{\phi})^{n}=\underbrace{ (rz_{\phi})\dots(rz_{\phi}) }_{ n }=r^{n}z_{n\phi}$

>[!note] Муавр верен при $n\leq0$ (проверить 0 и -1, а дальше применить обычную форму)

> [!example]- Сложный пример
> $$
> \begin{gathered}
> z_{\phi}^{n}=(\cos \phi+\sin \phi)^{n}=\sum\limits C_{n}^{k}\cos ^{k}\phi \sin ^{n-k}\phi\cdot i^{n-k}=\\=
> \cos ^{n}\phi-C_{n}^{2}\cos ^{n-2}\phi \sin ^{2} \phi+C_{n}^{4}\cos ^{n-4}\phi \sin ^{4}\phi+\dots+\\
> +i(C_{n}^{1}\cos ^{n-1}\phi \sin \phi-С_{n}^{3}\cos ^{n-3}\phi \sin ^{3}\phi+\dots)=\\
> =T^{(n)}_{1}(\cos \phi, \sin \phi)+iT_{2}^{(n)}(\cos \phi, \sin \phi)
> \end{gathered}
> $$
> Тогда 
> $$
> \begin{gathered}
> \cos n\phi=T_{1}^{(n)}(\cos \phi, \sin \phi)\\
> \sin n\phi=T_{2}^{(n)}(\cos \phi, \sin \phi)
> \end{gathered}
> $$

> [!example]- Пример полегче
> $$
> \begin{gathered}
> \sin \phi+\sin_{2}\phi+\dots+\sin(n\phi)=\mathrm{Im}(z_{\phi})+\dots+\mathrm{Im}(z_{n\phi})=\\
> =\mathrm{Im}(z_{\phi}+\dots+z^{n}_{\phi})=\mathrm{Im}\left( \frac{z_{\phi}^{n}-z_{\phi}}{z_{\phi}-1} \right)
> \end{gathered}
> $$