Если $\det_{1}$ и $\det_{2}$ удовл. [[Определитель|аксиомам]], то $\det_{1}=\det_{2}$
## Док-во

Пусть $\exists \det_{1}, \det_{2}$, удовл. акс. 1-3.

$\det_{1} E=\det_{2}E=1$

Д-м, что $\det_{1}(e_{i_{1}}|e_{i_{2}}\dots|e_{i_{n}})=\det_{2}(e_{i_{1}}|e_{i_{2}}\dots|e_{i_{n}})$

Если $i_{k}=i_{l}\implies \det_{1}(\dots)=\det_{2}(\dots)=0$
Иначе они все различн. $\implies \exists \pi: \pi(i_{k})=k$
$(e_{i, \pi(i)}|\dots)=E_{\pi}$

Тогда $\det_{i}(E_{\pi})=-\det_{i}(tE_{\pi})$ ($t$ — транспозиция, по кососим.) $\implies \det_{i}E_\pi=-\det E_{(t_{2}\dots t_{l})}=\dots=(-1)^{l}\det E$

Общий случай 
$$
\begin{gathered}
\det_{i}(c_{1},\dots c_{n})=\det\left( \sum\limits a_{i 1}e_{i},\dots \sum\limits a_{in}e_{i} \right)=\sum\limits a_{i1}\det \left( e_{i},\dots \sum\limits a_{jn}e_{j} \right)=\dots=\\
=\text{Л.К. } \det (e_{i_{1}},\dots e_{i_{n}})
\end{gathered}
$$
Значит $\det_{1}=\det_{2}$