$a_{n}, b_{n}$, $A_{n}:= a_{1}+\dots+a_{n},\ A_{0}:=0$

$$
\sum\limits_{k=1}^{n} a_{k}b_{k}=A_{n}b_{n}+\sum\limits_{k=1}^{n-1}A_{k}(b_{k}-b_{k-1})
$$
(см. [[Знакопеременный ряд]])
## Док-во

$a_{k}=A_{k}-A_{k-1}$

Тогда
$$
\begin{gathered}
\sum\limits_{k=1}^{n}a_{k}b_{k}=\sum\limits_{k=1}^{n}(A_{k}-A_{k-1})b_{k}=\sum\limits_{k=1}^{n}A_{k}b_{k}-\sum\limits_{j=1}^{n}A_{j-1}b_{j}\stackrel{[j-1=k]}{=}\sum\limits_{k=1}A_{k}b_{k}+\sum\limits_{k=1}^{n-1}A_{k}b_{k-1}=\\
=A_{n}b_{n}+\sum\limits_{k=1}^{n-1}A_{k}(b_{k}-b_{k-1})
\end{gathered}
$$
