$x_{n} = \left( 1+ \frac{a}{n} \right)^{n}, a\in \mathbb{R}$

1. $\{ x_{n} \}$ возр. при $n>-a$ (строго, если $a\ne 0$)
2. $\{ x_{n} \}$ огр. сверху
# Следствие

$\exists \lim\limits_{ n \to +\infty} x_n \in \mathbb{R}$ (монот. + огр.)
# Доказательство
## Пункт 1
$$
\begin{gathered}
\frac{x_{n}}{x_{n-1}}=\frac{\left( 1+\frac{a}{n} \right)^{n}}{\left( 1+\frac{a}{n-1} \right)^{n-1}} = \frac{(n+a)^{n}}{n^{n}}\cdot \frac{(n-1)^{n-1}}{(n-1+a)^{n-1}} = \left( \frac{(n+a)(n-1)}{n(n-1+a)} \right)^{n}\cdot \frac{n-1+a}{n-1} = \\ =\frac{n-1+a}{n-1}\left( 1+ \frac{-a}{n(n-1+a)} \right)^{n} \stackrel{Н.Б.}{\geq} \frac{n-1+a}{n-1}\left( 1+n\cdot \frac{-a}{n(n-1+a)} \right) =\\= \frac{n-1+a}{n-1}\cdot \frac{n-1+a-a}{n-1+a}=1
\end{gathered}
$$

$$
\frac{x_{n}}{x_{n-1}}\geq 1
$$
Проверим условие для Н.Б.:
$$
\begin{aligned}
\frac{-a}{n(n-1+a)}&>-1\\
\frac{a}{n(n-1+a)}&<1\\
a&<n(n-1+a)\\
n^{2}-n+an-a&>0\\
(n-1)(n+a)&>0
\end{aligned}
$$
## Пункт 2

$y_{n} = \left( 1+ \frac{-a}{n} \right)^{n}$ (может возр. при $n>a$)

$$
x_{n}y_{n} = \left( 1+\frac{a}{n} \right)^{n}\left( 1-\frac{a}{n} \right)^{n}=\left( 1-\frac{a^{2}}{n} \right)^{n} \leq 1
$$

НСНМ $x_{n}>0$ и $y_{n}>0$, значит $x_{n} \leq \frac{1}{y_{n}} \implies x_{n} \leq \frac{1}{y_{наим}} = const \implies \{ x_{n} \}$ — огр. сверху. 