1. $b\in \mathbb{N};\ b =n,n\in \mathbb{N}$
   $$a^{n}\stackrel{\text{def}}{=} \exp(n\ln a)=\exp(\underbrace{ \ln a+\dots+\ln a }_{ n })=\underbrace{ \exp(\ln a)\dots \exp(\ln a) }_{ n }=\underbrace{ a\cdot a\cdot\dots a }_{ n }=a^{n}$$
   2. $b \in \mathbb{Z};\ b = -n,\ n \in \mathbb{N}$
      $a^{-n}=\exp(-n\ln a)= \frac{1}{\exp(n\ln a)}=\frac{1}{a^{n}}$
  3. $a^{0}=1 \impliedby \exp(0)=1$
  4. $b \in \mathbb{Q}; b = \frac{m}{n},\ n \in \mathbb{N},\ m \in \mathbb{Z}$
     $$
\begin{gathered}
(a^{m/n})^{n}\stackrel{?}{=} a^{m}\\
a^{m/n}\stackrel{\text{def}}{=}\exp\left( \frac{m}{n} \ln a \right)\\
(a^{m/n})^{n}=\left( \exp\left( \frac{m}{n}\ln a \right) \right)^{n}=\exp\left( \cancel{ n }\cdot \frac{m}{\cancel{ n }}\ln a \right)\stackrel{\text{def}}{=}a^{n}
\end{gathered}
$$
