1. $e^{x}=\sum\limits_{n=0}^{+\infty} \frac{x^{n}}{n!}\ \forall x \in \mathbb{R}$
2. $\cos x = \sum\limits_{n=0}^{+\infty} (-1)^{n} \frac{x^{2n}}{(2n)!}\ \forall x \in \mathbb{R}$
3. $\sin x= \sum\limits_{n=0}^{+\infty} (-1)^{n} \frac{x^{2n+1}}{(2n+1)!}\ \forall x \in \mathbb{R}$

Ряды $\sum\limits_{n=0}^{+\infty} \frac{z^{n}}{n!},\ \sum\limits(-1)^{n} \frac{z^{2n}}{(2n)!}$ и $\sum\limits_{n=0}^{\infty} (-1)^{n} \frac{z^{2n+1}}{(2n+1)!}$ сх-ся при $\forall z \in \mathbb{C}$. Тогда
1. $\exp z:= \sum\limits_{n=0}^{\infty} \frac{z^{n}}{n!}$
2. $\cos z:= \sum\limits_{n=0}^{\infty} (-1)^{n} \frac{z^{2n}}{(2n)!}$
3. $\sin z:= \sum\limits_{n=0}^{\infty} (-1)^{n} \frac{z^{2n+1}}{(2n+1)!}$
>[!note] $\cos(-z)=\cos z$ и $\sin (-z)=-\sin z$

>[!note] **Формула Эйлера** $\exp(iz)=\cos z+i\sin z$

>[!note] $\cos z = \frac{\exp(iz)+\exp(-iz)}{2}$, $\sin z = \frac{\exp(iz)-\exp(iz)}{2}$

>[!question] Д-ть, что $\sin ^{2}z+\cos ^{2}z=1$

>[!question] Д-ть, что $\exp(z)\cdot \exp(w)=\exp(z+w)$

4. $\ln(1+x)=\sum\limits_{n=1}^{\infty} (-1)^{n-1} \frac{x^{n}}{n}$ при $x \in(-1, 1)$
>[!note]- Д-во
> $$
> \begin{gathered}
> (\ln(1+x))'=\frac{1}{1+x}\implies \ln(1+x)=\int\limits_{0}^{x} \frac{dt}{1+t}=\sum\limits_{n=0}^{\infty}(-1)^{n} t^{n}\,dt=\\=\sum\limits_{n=0}^{\infty}(-1)^{n}\int\limits_{0}^{x} t^{n}\,dt=\sum\limits_{n=0}^{\infty} (-1)^{n} \frac{x^{n+1}}{n+1}
> \end{gathered}
> $$
5. $\arctg x=\sum\limits_{n=0}^{\infty} (-1)^{n} \frac{x^{2n+1}}{2n+1}$ при $x \in(-1, 1)$
>[!note]- Док-во
> $$
> \begin{gathered}
> \arctg x = \int\limits_{0}^{x} \frac{dt}{1+t^{2}} = \int\limits_{0}^{x} \sum\limits_{n=0}^{\infty} (-1)^{n} t^{2n}\,dt=\sum\limits_{n=0}^{\infty} (-1)^{n}\int\limits_{0}^{x} t^{2n}\,dt=\sum\limits_{n=0}^{\infty} (-1)^{n} \frac{x^{2n+1}}{2n+1}
> \end{gathered}
> $$

>[!note]- **Сл-е**. $\frac{\pi}{4}=1-\frac{1}{3}+\frac{1}{5}-\frac{1}{7}+\dots$
> Ряд $\sum\limits_{n=0}^{\infty} (-1)^{n} \frac{x^{2n+1}}{2n+1}$ сх-ся при $x=1$. Тогда по th Абеля $f(1)=\lim\limits_{ x \to 1- }f(x)=\lim\limits_{ x \to 1- }\arctg(x)=\arctg1= \frac{\pi}{4}$

6. $\arcsin x=\sum\limits_{n=0}^{\infty} \frac{C_{2n}^{n}}{4^{n}}\cdot \frac{x^{2n+2}}{2n+1}$ при $x \in(-1, 1)$
>[!note]- Док-во
> (см. [[Теорема о рядах с нисходящим факториалом]])
> $$
> \arcsin x=\int\limits_{0}^{x} \frac{dt}{\sqrt{1-t^{2}}} =\int\limits_{0}^{x} \sum\limits_{n=0}^{\infty} \frac{C_{2n}^{n}}{4^{n}} t^{2n}\,dt=\sum\limits_{n=0}^{\infty} \frac{C_{2n}^{n}}{4^{n}} \cdot \frac{x^{2n+1}}{2n+1}
> $$
